[Lambek] updated project code

lambek/LambekScript.sml
@@ -1,123 +1,192 @@
 (*
- * A HOL Toolkit for Lambek Calculus & Categorial Type Logics
+ * Formalized Lambek Calculus in Higher Order Logic (HOL4)
  *
- * (based on `A Coq Toolkit for Lambek Calculus` (https://github.com/coq-contribs/lambek)
+ *  (based on https://github.com/coq-contribs/lambek)
  *
+ * Copyright 2002-2003  Houda ANOUN and Pierre Casteran, LaBRI/INRIA.
  * Copyright 2016-2017  University of Bologna, Italy (Author: Chun Tian)
- *
- * Licensed under the Apache License, Version 2.0 (the "License");
- * you may not use this file except in compliance with the License.
- * You may obtain a copy of the License at
- *
- *  http://www.apache.org/licenses/LICENSE-2.0
- *
- * THIS CODE IS PROVIDED *AS IS* BASIS, WITHOUT WARRANTIES OR CONDITIONS OF ANY
- * KIND, EITHER EXPRESS OR IMPLIED, INCLUDING WITHOUT LIMITATION ANY IMPLIED
- * WARRANTIES OR CONDITIONS OF TITLE, FITNESS FOR A PARTICULAR PURPOSE,
- * MERCHANTABLITY OR NON-INFRINGEMENT.
- * See the Apache 2 License for the specific language governing permissions and
- * limitations under the License.
  *)
+
+(* This program is free software; you can redistribute it and/or      *)
+(* modify it under the terms of the GNU Lesser General Public License *)
+(* as published by the Free Software Foundation; either version 2.1   *)
+(* of the License, or (at your option) any later version.             *)
+(*                                                                    *)
+(* This program is distributed in the hope that it will be useful,    *)
+(* but WITHOUT ANY WARRANTY; without even the implied warranty of     *)
+(* MERCHANTABILITY or FITNESS FOR A PARTICULAR PURPOSE.  See the      *)
+(* GNU General Public License for more details.                       *)
+(*                                                                    *)
+(* You should have received a copy of the GNU Lesser General Public   *)
+(* License along with this program; if not, write to the Free         *)
+(* Software Foundation, Inc., 51 Franklin St, Fifth Floor, Boston, MA *)
+(* 02110-1301 USA                                                     *)
 
 open HolKernel Parse boolLib bossLib;
 
-open relationTheory listTheory arithmeticTheory;
+open pred_setTheory pairTheory listTheory arithmeticTheory integerTheory;
+open relationTheory;
+
+(* Set PAT_X_ASSUM to PAT_ASSUM if it's not defined yet *)
+local
+    val PAT_X_ASSUM = PAT_ASSUM;
+    val qpat_x_assum = Q.PAT_ASSUM;
+    open Tactical
+in
+    val PAT_X_ASSUM = PAT_X_ASSUM;
+    val qpat_x_assum = qpat_x_assum
+end;
 
 val _ = new_theory "Lambek";
 
-(*** Module: Form ***)
+(******************************************************************************)
+(*                                                                            *)
+(*                              Module: Form                                  *)
+(*                                                                            *)
+(******************************************************************************)
 
-val _ = Datatype `Form = Atom 'a | Slash Form Form | Backslash Form Form | Dot Form Form`;
+val _ = Datatype `Form = At 'a | Slash Form Form | Backslash Form Form | Dot Form Form`;
 
-(* or val _ = overload_on ("*", Term `Dot`); *)
-val _ = set_mapped_fixity { fixity = Infix(NONASSOC, 450), tok = ".", term_name = "Dot" };
-val _ = set_mapped_fixity { fixity = Infix(LEFT, 1000), tok = "/", term_name = "Slash" };
-val _ = set_mapped_fixity { fixity = Infix(RIGHT, 1500), tok = "\\", term_name = "Backslash" };
+val _ = overload_on ("*", ``Dot``); (* \HOLTokenProd *)
+val _ = overload_on ("/", ``Slash``);
+val _ = overload_on ("\\\\", ``Backslash``);
+val _ = set_fixity "\\\\" (Infixr 1500);
+val _ = TeX_notation { hol = "\\\\", TeX = ("\\HOLTokenBackslash", 1) };
 
-(** The arrow relationship and its extensions (like associativity, commutativity  etc.) **)
+val Form_induction = TypeBase.induction_of ``:'a Form``;
+val Form_nchotomy  = TypeBase.nchotomy_of ``:'a Form``;
+val Form_distinct  = TypeBase.distinct_of ``:'a Form``;
+val Form_distinct' = save_thm ("Form_distinct'", GSYM Form_distinct);
+val Form_11        = TypeBase.one_one_of ``:'a Form``;
 
 val _ = type_abbrev ("arrow_extension", ``:'a Form -> 'a Form -> bool``);
 
-val _ = overload_on("add_extension", ``relation$RUNION``);
+(* Rules of Lambek's "Syntactic Calculus" (non-associative + extension) *)
+val (arrow_rules, arrow_ind, arrow_cases) = Hol_reln `
+    (!X A. arrow X A A) /\						(* one *)
+    (!X A B C. arrow X (Dot A B) C ==> arrow X A (Slash C B)) /\	(* beta *)
+    (!X A B C. arrow X A (Slash C B) ==> arrow X (Dot A B) C) /\	(* beta' *)
+    (!X A B C. arrow X (Dot A B) C ==> arrow X B (Backslash A C)) /\	(* gamma *)
+    (!X A B C. arrow X B (Backslash A C) ==> arrow X (Dot A B) C) /\	(* gamma' *)
+    (!X A B C. arrow X A B /\ arrow X B C ==> arrow X A C) /\		(* comp *)
+    (!(X :'a arrow_extension) A B. X A B ==> arrow X A B) `;		(* arrow_plus *)
 
-val extends_def = Define `extends X X' = X RSUBSET X'`;
+local
+    val list = CONJUNCTS arrow_rules
+in
+    val one         = save_thm ("one",         List.nth (list, 0))
+    and beta        = save_thm ("beta",        List.nth (list, 1))
+    and beta'       = save_thm ("beta'",       List.nth (list, 2))
+    and gamma       = save_thm ("gamma",       List.nth (list, 3))
+    and gamma'      = save_thm ("gamma'",      List.nth (list, 4))
+    and comp        = save_thm ("comp",        List.nth (list, 5))
+    and arrow_plus  = save_thm ("arrow_plus",  List.nth (list, 6))
+end;
+
+val beta_EQ = store_thm ("beta_EQ",
+  ``!X A B C. arrow X A (Slash C B) = arrow X (Dot A B) C``,
+    REPEAT STRIP_TAC
+ >> EQ_TAC
+ >| [ REWRITE_TAC [beta'],
+      REWRITE_TAC [beta] ]);
+
+val gamma_EQ = store_thm ("gamma_EQ",
+  ``!X A B C. arrow X B (Backslash A C) = arrow X (Dot A B) C``,
+    REPEAT STRIP_TAC
+ >> EQ_TAC
+ >| [ REWRITE_TAC [gamma'],
+      REWRITE_TAC [gamma] ]);
+
+val arrow_transitive = store_thm (
+   "arrow_transitive", ``!X. transitive (arrow X)``,
+   REWRITE_TAC [transitive_def, comp]);
+
+val arrow_reflexive = store_thm (
+   "arrow_reflexive", ``!X. reflexive (arrow X)``,
+   REWRITE_TAC [reflexive_def, one]);
+
+(** The arrow relationship and its extensions (like associativity, commutativity  etc.) **)
+
+val _ = overload_on("add_extension", ``relation$RUNION``);
+(* X extends (to) X', or X is extended to X' *)
+val _ = overload_on("extends", ``relation$RSUBSET``);
 
 val no_extend = store_thm ("no_extend", ``!X. extends X X``,
-    RW_TAC bool_ss [extends_def, RSUBSET]);
+    RW_TAC bool_ss [RSUBSET]);
 
 val add_extend_l = store_thm ("add_extend_l", ``!X X'. extends X (add_extension X X')``,
-    RW_TAC bool_ss [extends_def, RSUBSET, RUNION]);
+    RW_TAC bool_ss [RSUBSET, RUNION]);
 
 val add_extend_r = store_thm ("add_extend_r", ``!X X'. extends X' (add_extension X X')``,
-    RW_TAC bool_ss [extends_def, RSUBSET, RUNION]);
+    RW_TAC bool_ss [RSUBSET, RUNION]);
 
 val extends_trans = store_thm ("extends_trans",
   ``!X Y Z. extends X Y /\ extends Y Z ==> extends X Z``,
-    RW_TAC bool_ss [extends_def, RSUBSET]);
+    RW_TAC bool_ss [RSUBSET]);
 
-val extends_transitive = store_thm ("extends_trans", ``transitive extends``,
+val extends_transitive = store_thm (
+   "extends_transitive", ``transitive extends``,
     REWRITE_TAC [transitive_def, extends_trans]);
-
-(* Rules of Lambek's syntactic calculus (non-associative) *)
-val (Arrow_rules, Arrow_ind, _) = Hol_reln `
-    (!X A. Arrow X A A) /\						(* a  / one    *)
-    (!X A B C. Arrow X (Dot A B) C ==> Arrow X A (Slash C B)) /\	(* c  / beta   *)
-    (!X A B C. Arrow X A (Slash C B) ==> Arrow X (Dot A B) C) /\	(* d  / beta'  *)
-    (!X A B C. Arrow X (Dot A B) C ==> Arrow X B (Backslash A C)) /\	(* c' / gamma  *)
-    (!X A B C. Arrow X B (Backslash A C) ==> Arrow X (Dot A B) C) /\	(* d' / gamma' *)
-    (!X A B C. Arrow X A B /\ Arrow X B C ==> Arrow X A C) /\		(* e  / comp   *)
-    (!X A B. X A B ==> Arrow X A B)`;					(* arrow_plus  *)
-
-val [one, beta, beta', gamma, gamma', comp, arrow_plus] = CONJ_LIST 7 Arrow_rules;
 
 (** most popular extensions **)
 
-val NL_def = Define `NL = EMPTY_REL`;
+val NL_def = Define `(NL :'a arrow_extension) = EMPTY_REL`;
 
-val (L_rules, _ , _) = Hol_reln `
+(* L is defined by two rules, and it's reflexitive *)
+val (L_rules, L_ind, L_cases) = Hol_reln `
     (!A B C. L (Dot A (Dot B C)) (Dot (Dot A B) C)) /\
     (!A B C. L (Dot (Dot A B) C) (Dot A (Dot B C)))`;
 
-val [L_rule_rl, L_rule_lr] = CONJ_LIST 2 L_rules;
+local
+    val list = CONJUNCTS L_rules
+in
+    val L_rule_rl = save_thm ("L_rule_rl", List.nth (list, 0))
+    and L_rule_lr = save_thm ("L_rule_lr", List.nth (list, 1))
+end;
 
-val (NLP_rules, _, _) = Hol_reln `(!A B. NLP (Dot A B) (Dot B A))`;
+(* NLP is defined by only one rule, it's reflexitive too. *)
+val (NLP_rules, NLP_ind, NLP_cases) = Hol_reln `
+    (!A B. NLP (Dot A B) (Dot B A))`;
 
 val LP_def = Define `LP = add_extension NLP L`;
 
-val NL_X = store_thm ("NL_X", ``!X. extends NL X``,
-    RW_TAC bool_ss [extends_def, NL_def, EMPTY_REL_DEF, RSUBSET]);
+val NLextendsAll = store_thm (
+   "NLextendsAll", ``!X. extends NL X``,
+    RW_TAC bool_ss [NL_def, EMPTY_REL_DEF, RSUBSET]);
 
-val NLP_LP = store_thm ("NLP_LP", ``extends NLP LP``,
+val NLPextendsLP = store_thm ("NLPextendsLP", ``extends NLP LP``,
     REWRITE_TAC [LP_def, add_extend_l]);
 
-val L_LP = store_thm ("L_LP", ``extends L LP``,
+val LextendsLP = store_thm ("LextendsLP", ``extends L LP``,
     REWRITE_TAC [LP_def, add_extend_r]);
 
 (* Some derived rules for arrow.
-   Note: all theorems here can be simply proved by PROVE_TAC [Arrow_rules]. *)
+   Note: all theorems here can be simply proved by PROVE_TAC [arrow_rules]. *)
 
 val Dot_mono_right = store_thm ("Dot_mono_right",
-  ``!X A B B'. Arrow X B' B ==> Arrow X (Dot A B') (Dot A B)``,
+  ``!X A B B'. arrow X B' B ==> arrow X (Dot A B') (Dot A B)``,
     REPEAT STRIP_TAC
  >> MATCH_MP_TAC gamma'
  >> MATCH_MP_TAC comp
  >> Q.EXISTS_TAC `B`
  >> CONJ_TAC
- >| [ ASM_REWRITE_TAC [],
-      MATCH_MP_TAC gamma >> RW_TAC bool_ss [one] ]);
+ >- ASM_REWRITE_TAC []
+ >> MATCH_MP_TAC gamma
+ >> RW_TAC bool_ss [one]);
 
 val Dot_mono_left = store_thm ("Dot_mono_left",
-  ``!X A B A'. Arrow X A' A ==> Arrow X (Dot A' B) (Dot A B)``,
+  ``!X A B A'. arrow X A' A ==> arrow X (Dot A' B) (Dot A B)``,
     REPEAT STRIP_TAC
  >> MATCH_MP_TAC beta'
  >> MATCH_MP_TAC comp
  >> Q.EXISTS_TAC `A`
  >> CONJ_TAC
- >| [ ASM_REWRITE_TAC [],
-      MATCH_MP_TAC beta >> RW_TAC bool_ss [one] ]);
+ >- ASM_REWRITE_TAC []
+ >> MATCH_MP_TAC beta
+ >> RW_TAC bool_ss [one]);
 
 val Dot_mono = store_thm ("Dot_mono",
-  ``!X A B C D. Arrow X A C /\ Arrow X B D ==> Arrow X (Dot A B) (Dot C D)``,
+  ``!X A B C D. arrow X A C /\ arrow X B D ==> arrow X (Dot A B) (Dot C D)``,
     REPEAT STRIP_TAC
  >> MATCH_MP_TAC comp
  >> EXISTS_TAC ``(Dot C B)``
@@ -126,181 +195,200 @@ val Dot_mono = store_thm ("Dot_mono",
       MATCH_MP_TAC Dot_mono_right >> RW_TAC bool_ss [] ]);
 
 val Slash_mono_left = store_thm ("Slash_mono_left",
-  ``!X C B C'. Arrow X C' C ==> Arrow X (Slash C' B) (Slash C B)``,
+  ``!X C B C'. arrow X C' C ==> arrow X (Slash C' B) (Slash C B)``,
     REPEAT STRIP_TAC
  >> MATCH_MP_TAC beta
  >> MATCH_MP_TAC comp
  >> Q.EXISTS_TAC `C'`
  >> CONJ_TAC
- >| [ MATCH_MP_TAC beta' >> RW_TAC bool_ss [one], RW_TAC bool_ss [] ]);
+ >| [ MATCH_MP_TAC beta' >> RW_TAC bool_ss [one],
+      RW_TAC bool_ss [] ]);
 
 val Slash_antimono_right = store_thm ("Slash_antimono_right",
-  ``!X C B B'. Arrow X B' B ==> Arrow X (Slash C B) (Slash C B')``,
+  ``!X C B B'. arrow X B' B ==> arrow X (Slash C B) (Slash C B')``,
     REPEAT STRIP_TAC
  >> MATCH_MP_TAC beta
  >> MATCH_MP_TAC gamma'
  >> MATCH_MP_TAC comp
  >> Q.EXISTS_TAC `B`
  >> CONJ_TAC
- >| [ ASM_REWRITE_TAC [],
-      MATCH_MP_TAC gamma >> MATCH_MP_TAC beta' >> RW_TAC bool_ss [one] ]);
+ >- ASM_REWRITE_TAC []
+ >> MATCH_MP_TAC gamma
+ >> MATCH_MP_TAC beta'
+ >> RW_TAC bool_ss [one]);
 
 val Backslash_antimono_left = store_thm ("Backslash_antimono_left",
-  ``!X A C A'. Arrow X A A' ==> Arrow X (Backslash A' C) (Backslash A C)``,
+  ``!X A C A'. arrow X A A' ==> arrow X (Backslash A' C) (Backslash A C)``,
     REPEAT STRIP_TAC
  >> MATCH_MP_TAC gamma
  >> MATCH_MP_TAC beta'
  >> MATCH_MP_TAC comp
  >> Q.EXISTS_TAC `A'`
  >> CONJ_TAC
- >| [ ASM_REWRITE_TAC [],
-      MATCH_MP_TAC beta >> MATCH_MP_TAC gamma' >> RW_TAC bool_ss [one] ]);
+ >- ASM_REWRITE_TAC []
+ >> MATCH_MP_TAC beta
+ >> MATCH_MP_TAC gamma'
+ >> RW_TAC bool_ss [one]);
 
 val Backslash_mono_right = store_thm ("Backslash_mono_right",
-  ``!X A C C'. Arrow X C' C ==> Arrow X (Backslash A C') (Backslash A C)``,
+  ``!X A C C'. arrow X C' C ==> arrow X (Backslash A C') (Backslash A C)``,
     REPEAT STRIP_TAC
  >> MATCH_MP_TAC gamma
  >> MATCH_MP_TAC comp
  >> Q.EXISTS_TAC `C'`
  >> CONJ_TAC
- >| [ MATCH_MP_TAC beta' >> MATCH_MP_TAC beta >>
-      MATCH_MP_TAC gamma' >> RW_TAC bool_ss [one],
+ >| [ MATCH_MP_TAC beta' \\
+      MATCH_MP_TAC beta \\
+      MATCH_MP_TAC gamma' \\
+      RW_TAC bool_ss [one],
       ASM_REWRITE_TAC [] ]);
 
 val mono_X = store_thm ("mono_X",
-  ``!X' X A B. Arrow X A B ==> extends X X' ==> Arrow X' A B``,
+  ``!X' X A B. arrow X A B ==> extends X X' ==> arrow X' A B``,
     GEN_TAC
- >> HO_MATCH_MP_TAC Arrow_ind (* or stronger: Induct_on `Arrow` *)
- >> REPEAT STRIP_TAC (* 7 sub-goals *)
- >| [ REWRITE_TAC [one],
-      RW_TAC bool_ss [beta],
-      RW_TAC bool_ss [beta'],
-      RW_TAC bool_ss [gamma],
-      RW_TAC bool_ss [gamma'],
-      PROVE_TAC [comp],
-      PROVE_TAC [arrow_plus, extends_def, RSUBSET] ]);
+ >> Induct_on `arrow`
+ >> REPEAT STRIP_TAC (* 7 sub-goals here *)
+ >- REWRITE_TAC [one]
+ >- RW_TAC bool_ss [beta]
+ >- RW_TAC bool_ss [beta']
+ >- RW_TAC bool_ss [gamma]
+ >- RW_TAC bool_ss [gamma']
+ >- PROVE_TAC [comp]
+ >> PROVE_TAC [arrow_plus, RSUBSET]);
 
-val pi = store_thm ("pi", ``!X. extends NLP X ==> (!A B. Arrow X (Dot A B) (Dot B A))``,
+val pi = store_thm ("pi",
+  ``!X. extends NLP X ==> !A B. arrow X (Dot A B) (Dot B A)``,
     REPEAT STRIP_TAC
  >> `NLP (Dot A B) (Dot B A)` by REWRITE_TAC [NLP_rules]
- >> `Arrow NLP (Dot A B) (Dot B A)` by RW_TAC bool_ss [arrow_plus]
+ >> `arrow NLP (Dot A B) (Dot B A)` by RW_TAC bool_ss [arrow_plus]
  >> PROVE_TAC [mono_X]);
 
-val pi_NLP = store_thm ("pi_NLP", ``!A B. Arrow NLP (Dot A B) (Dot B A)``,
+val pi_NLP = store_thm ("pi_NLP", ``!A B. arrow NLP (Dot A B) (Dot B A)``,
     MATCH_MP_TAC pi
  >> REWRITE_TAC [no_extend]);
 
-val pi_LP = store_thm ("pi_LP", ``!A B. Arrow LP (Dot A B) (Dot B A)``,
+val pi_LP = store_thm ("pi_LP", ``!A B. arrow LP (Dot A B) (Dot B A)``,
     MATCH_MP_TAC pi
- >> REWRITE_TAC [NLP_LP]);
+ >> REWRITE_TAC [NLPextendsLP]);
 
-(* original name: alpha in Coq version *)
-val aleph = store_thm ("aleph",
-  ``!X. extends L X ==> (!A B C. Arrow X (Dot A (Dot B C)) (Dot (Dot A B) C))``,
+val alfa = store_thm ("alfa",
+  ``!X. extends L X ==> !A B C. arrow X (Dot A (Dot B C)) (Dot (Dot A B) C)``,
     REPEAT STRIP_TAC
- >> `L (Dot A (Dot B C)) (Dot (Dot A B) C)` by REWRITE_TAC [L_rule_rl]
- >> `Arrow L (Dot A (Dot B C)) (Dot (Dot A B) C)` by RW_TAC bool_ss [arrow_plus]
+ >> `L (Dot A (Dot B C)) (Dot (Dot A B) C)`
+	by REWRITE_TAC [L_rule_rl]
+ >> `arrow L (Dot A (Dot B C)) (Dot (Dot A B) C)`
+	by RW_TAC bool_ss [arrow_plus]
  >> PROVE_TAC [mono_X]);
 
-val aleph_L = store_thm ("aleph_L", ``!A B C. Arrow L (Dot A (Dot B C)) (Dot (Dot A B) C)``,
-    MATCH_MP_TAC aleph
+val alfa_L = store_thm ("alfa_L",
+  ``!A B C. arrow L (Dot A (Dot B C)) (Dot (Dot A B) C)``,
+    MATCH_MP_TAC alfa
  >> REWRITE_TAC [no_extend]);
 
-val aleph_LP = store_thm ("aleph_LP", ``!A B C. Arrow LP (Dot A (Dot B C)) (Dot (Dot A B) C)``,
-    MATCH_MP_TAC aleph
- >> REWRITE_TAC [L_LP]);
+val alfa_LP = store_thm ("alfa_LP",
+  ``!A B C. arrow LP (Dot A (Dot B C)) (Dot (Dot A B) C)``,
+    MATCH_MP_TAC alfa
+ >> REWRITE_TAC [LextendsLP]);
 
-val aleph' = store_thm ("aleph'",
-  ``!X. extends L X ==> (!A B C. Arrow X (Dot (Dot A B) C) (Dot A (Dot B C)))``,
+val alfa' = store_thm ("alfa'",
+  ``!X. extends L X ==> !A B C. arrow X (Dot (Dot A B) C) (Dot A (Dot B C))``,
     REPEAT STRIP_TAC
  >> `L (Dot (Dot A B) C) (Dot A (Dot B C))` by REWRITE_TAC [L_rule_lr]
- >> `Arrow L (Dot (Dot A B) C) (Dot A (Dot B C))` by RW_TAC bool_ss [arrow_plus]
+ >> `arrow L (Dot (Dot A B) C) (Dot A (Dot B C))` by RW_TAC bool_ss [arrow_plus]
  >> PROVE_TAC [mono_X]);
 
-val aleph'_L = store_thm ("aleph'_L", ``!A B C. Arrow L (Dot (Dot A B) C) (Dot A (Dot B C))``,
-    MATCH_MP_TAC aleph'
+val alfa'_L = store_thm ("alfa'_L",
+  ``!A B C. arrow L (Dot (Dot A B) C) (Dot A (Dot B C))``,
+    MATCH_MP_TAC alfa'
  >> REWRITE_TAC [no_extend]);
 
-val aleph'_LP = store_thm ("aleph'_LP", ``!A B C. Arrow LP (Dot (Dot A B) C) (Dot A (Dot B C))``,
-    MATCH_MP_TAC aleph'
- >> REWRITE_TAC [L_LP]);
+val alfa'_LP = store_thm ("alfa'_LP",
+  ``!A B C. arrow LP (Dot (Dot A B) C) (Dot A (Dot B C))``,
+    MATCH_MP_TAC alfa'
+ >> REWRITE_TAC [LextendsLP]);
 
-(* Arrow for Standard (full) Lambek calculus, here we recover all lemmas in Lambek (1958) *)
+(******************************************************************************)
+(*                                                                            *)
+(*                            L rules                                         *)
+(*                                                                            *)
+(******************************************************************************)
 
-val arrow_def = Define `arrow = Arrow L`;
+val L_a = store_thm ("L_a", ``!x. arrow L x x``, REWRITE_TAC [one]);
+val L_b = store_thm ("L_b",  ``!x y z. arrow L (Dot (Dot x y) z) (Dot x (Dot y z))``,
+    REWRITE_TAC [alfa'_L]);
+val L_b' = store_thm ("L_b'", ``!x y z. arrow L (Dot x (Dot y z)) (Dot (Dot x y) z)``,
+    REWRITE_TAC [alfa_L, alfa'_L]);
+val L_c  = store_thm ("L_c",  ``!x y z. arrow L (Dot x y) z ==> arrow L x (Slash z y)``,
+    REWRITE_TAC [beta]);
+val L_c' = store_thm ("L_c'", ``!x y z. arrow L (Dot x y) z ==> arrow L y (Backslash x z)``,
+    REWRITE_TAC [gamma]);
+val L_d  = store_thm ("L_d",  ``!x y z. arrow L x (Slash z y) ==> arrow L (Dot x y) z``,
+    REWRITE_TAC [beta']);
+val L_d' = store_thm ("L_d'", ``!x y z. arrow L y (Backslash x z) ==> arrow L (Dot x y) z``,
+    REWRITE_TAC [gamma']);
+val L_e  = store_thm ("L_e",  ``!x y z. arrow L x y /\ arrow L y z ==> arrow L x z``,
+    REWRITE_TAC [comp]);
 
-val _ = set_mapped_fixity { fixity = Infix(NONASSOC, 450), tok = "-->", term_name = "arrow" };
-val _ = Unicode.unicode_version {u = UnicodeChars.rightarrow, tmnm = "arrow"};
-
-val L_a = store_thm ("L_a", ``!x. arrow x x``, REWRITE_TAC [arrow_def, one]);
-val L_b = store_thm ("L_b",  ``!x y z. arrow (Dot (Dot x y) z) (Dot x (Dot y z))``,
-    REWRITE_TAC [arrow_def, aleph'_L]);
-val L_b' = store_thm ("L_b'", ``!x y z. arrow (Dot x (Dot y z)) (Dot (Dot x y) z)``,
-    REWRITE_TAC [arrow_def, aleph_L, aleph'_L]);
-val L_c  = store_thm ("L_c",  ``!x y z. arrow (Dot x y) z ==> arrow x (Slash z y)``,
-    REWRITE_TAC [arrow_def, beta]);
-val L_c' = store_thm ("L_c'", ``!x y z. arrow (Dot x y) z ==> arrow y (Backslash x z)``,
-    REWRITE_TAC [arrow_def, gamma]);
-val L_d  = store_thm ("L_d",  ``!x y z. arrow x (Slash z y) ==> arrow (Dot x y) z``,
-    REWRITE_TAC [arrow_def, beta']);
-val L_d' = store_thm ("L_d'", ``!x y z. arrow y (Backslash x z) ==> arrow (Dot x y) z``,
-    REWRITE_TAC [arrow_def, gamma']);
-val L_e  = store_thm ("L_e",  ``!x y z. arrow x y /\ arrow y z ==> arrow x z``,
-    REWRITE_TAC [arrow_def, comp]);
-
-val arrow_rules = LIST_CONJ [L_a, L_b, L_b', L_c, L_c', L_d, L_d', L_e];
+val L_arrow_rules = save_thm (
+   "L_arrow_rules", LIST_CONJ [L_a, L_b, L_b', L_c, L_c', L_d, L_d', L_e]);
 
 local
-  val t = PROVE_TAC [arrow_rules]
+  val t = PROVE_TAC [L_arrow_rules]
 in
-  val L_f  = store_thm ("L_f",  ``!x y. arrow x (Slash (Dot x y) y)``, t)
-  and L_g  = store_thm ("L_g",  ``!y z. arrow (Dot (Slash z y) y) z``, t)
-  and L_h  = store_thm ("L_h",  ``!y z. arrow y (Backslash (Slash z y) z)``, t)
-  and L_i  = store_thm ("L_i",  ``!x y z. arrow (Dot (Slash z y) (Slash y x)) (Slash z x)``, t)
-  and L_j  = store_thm ("L_j",  ``!x y z. arrow (Slash z y) (Slash (Slash z x) (Slash y x))``, t)
-  and L_k  = store_thm ("L_k",  ``!x y z. arrow (Slash (Backslash x y) z) (Backslash x (Slash y z))``, t)
-  and L_k' = store_thm ("L_k'", ``!x y z. arrow (Backslash x (Slash y z)) (Slash (Backslash x y) z)``, t)
-  and L_l  = store_thm ("L_l",  ``!x y z. arrow (Slash (Slash x y) z) (Slash x (Dot z y))``, t)
-  and L_l' = store_thm ("L_l'", ``!x y z. arrow (Slash x (Dot z y)) (Slash (Slash x y) z)``, t)
-  and L_m  = store_thm ("L_m",  ``!x x' y y'. arrow x x' /\ arrow y y'
-					  ==> arrow (Dot x y) (Dot x' y')``, t)
-  and L_n  = store_thm ("L_n",  ``!x x' y y'. arrow x x' /\ arrow y y'
-					  ==> arrow (Slash x y') (Slash x' y)``, t);
+  val L_f  = store_thm ("L_f",  ``!x y. arrow L x (Slash (Dot x y) y)``, t)
+  and L_g  = store_thm ("L_g",  ``!y z. arrow L (Dot (Slash z y) y) z``, t)
+  and L_h  = store_thm ("L_h",  ``!y z. arrow L y (Backslash (Slash z y) z)``, t)
+  and L_i  = store_thm ("L_i",  ``!x y z. arrow L (Dot (Slash z y) (Slash y x)) (Slash z x)``, t)
+  and L_j  = store_thm ("L_j",  ``!x y z. arrow L (Slash z y) (Slash (Slash z x) (Slash y x))``, t)
+  and L_k  = store_thm ("L_k",  ``!x y z. arrow L (Slash (Backslash x y) z) (Backslash x (Slash y z))``, t)
+  and L_k' = store_thm ("L_k'", ``!x y z. arrow L (Backslash x (Slash y z)) (Slash (Backslash x y) z)``, t)
+  and L_l  = store_thm ("L_l",  ``!x y z. arrow L (Slash (Slash x y) z) (Slash x (Dot z y))``, t)
+  and L_l' = store_thm ("L_l'", ``!x y z. arrow L (Slash x (Dot z y)) (Slash (Slash x y) z)``, t)
+  and L_m  = store_thm ("L_m",  ``!x x' y y'. arrow L x x' /\ arrow L y y'
+					  ==> arrow L (Dot x y) (Dot x' y')``, t)
+  and L_n  = store_thm ("L_n",  ``!x x' y y'. arrow L x x' /\ arrow L y y'
+					  ==> arrow L (Slash x y') (Slash x' y)``, t);
 
-  val arrow_rules_ex = LIST_CONJ [L_f, L_g, L_h, L_i, L_j, L_k, L_k', L_l, L_l', L_m, L_n]
+  val L_arrow_rules_ex = save_thm (
+     "L_arrow_rules_ex", LIST_CONJ [L_f, L_g, L_h, L_i, L_j, L_k, L_k', L_l, L_l', L_m, L_n])
 end;
 
 local
   val t = PROVE_TAC [L_a, L_c, L_c', L_d, L_d', L_e] (* L_b and L_b' are not used *)
 in
   val L_dot_mono_r = store_thm ("L_dot_mono_r",
-      ``!A B B'. arrow B B' ==> arrow (Dot A B) (Dot A B')``, t)
+      ``!A B B'. arrow L B B' ==> arrow L (Dot A B) (Dot A B')``, t)
   and L_dot_mono_l = store_thm ("L_dot_mono_l",
-      ``!A B A'. arrow A A' ==> arrow (Dot A B) (Dot A' B)``, t)
+      ``!A B A'. arrow L A A' ==> arrow L (Dot A B) (Dot A' B)``, t)
   and L_slash_mono_l = store_thm ("L_slash_mono_l",
-      ``!C B C'. arrow C C' ==> arrow (Slash C B) (Slash C' B)``, t)
+      ``!C B C'. arrow L C C' ==> arrow L (Slash C B) (Slash C' B)``, t)
   and L_slash_antimono_r = store_thm ("L_slash_antimono_r",
-      ``!C B B'. arrow B B' ==> arrow (Slash C B') (Slash C B)``, t)
+      ``!C B B'. arrow L B B' ==> arrow L (Slash C B') (Slash C B)``, t)
   and L_backslash_antimono_l = store_thm ("L_backslash_antimono_l",
-      ``!A C A'. arrow A A' ==> arrow (Backslash A' C) (Backslash A C)``, t)
+      ``!A C A'. arrow L A A' ==> arrow L (Backslash A' C) (Backslash A C)``, t)
   and L_backslash_mono_r = store_thm ("L_backslash_mono_r",
-      ``!A C C'. arrow C C' ==> arrow (Backslash A C) (Backslash A C')``, t);
+      ``!A C C'. arrow L C C' ==> arrow L (Backslash A C) (Backslash A C')``, t);
 
-  val arrow_rules_mono = LIST_CONJ [L_dot_mono_r, L_dot_mono_l,
-				    L_slash_mono_l, L_slash_antimono_r,
-				    L_backslash_antimono_l, L_backslash_mono_r]
+  val L_arrow_rules_mono = save_thm (
+     "L_arrow_rules_mono",
+      LIST_CONJ [L_dot_mono_r, L_dot_mono_l,
+		 L_slash_mono_l, L_slash_antimono_r,
+		 L_backslash_antimono_l, L_backslash_mono_r])
 end;
 
-(*** Module: Terms ***)
+(******************************************************************************)
+(*                                                                            *)
+(*                              Module: Terms                                 *)
+(*                                                                            *)
+(******************************************************************************)
 
 val _ = Datatype `Term = OneForm ('a Form) | Comma Term Term`;
 
-(*
-val _ = add_rule { term_name = "Comma", fixity = Infix(LEFT, 500),
-		   pp_elements = [HardSpace 0, TOK "," , BreakSpace(1,0)],
-		   paren_style = Always,
-		   block_style = (AroundEachPhrase, (PP.INCONSISTENT, 0)) };
-*)
+val Term_induction = TypeBase.induction_of ``:'a Term``;
+val Term_nchotomy  = TypeBase.nchotomy_of ``:'a Term``;
+val Term_distinct  = TypeBase.distinct_of ``:'a Term``;
+val Term_distinct' = save_thm ("Term_distinct'", GSYM Term_distinct);
+val Term_11        = TypeBase.one_one_of ``:'a Term``;
 
 val _ = type_abbrev ("gentzen_extension", ``:'a Term -> 'a Term -> bool``);
 
@@ -309,63 +397,61 @@ val deltaTranslation_def = Define `
    (deltaTranslation (OneForm f) = f) /\
    (deltaTranslation (Comma t1 t2) = Dot (deltaTranslation t1) (deltaTranslation t2))`;
 
-(* Definition of the relation that connects arrow_extension with gentzen_extension *)
-val implements_def = Define
-   `implements (X:'a arrow_extension) (E:'a gentzen_extension) =
-    (!(A:'a Term) (B:'a Term). E A B = X (deltaTranslation A) (deltaTranslation B))`;
+val deltaTranslationOneForm = store_thm (
+   "deltaTranslationOneForm[simp]",
+  ``deltaTranslation (OneForm f) = f``, RW_TAC std_ss [deltaTranslation_def]);
 
-(* NL Sequent extension, an empty relation actually *)
-val NL_Sequent_def = Define `NL_Sequent A B = NL (deltaTranslation A) (deltaTranslation B)`;
+val deltaTranslationComma = store_thm (
+   "deltaTranslationComma[simp]",
+  ``deltaTranslation (Comma t1 t2) = Dot (deltaTranslation t1) (deltaTranslation t2)``,
+    RW_TAC std_ss [deltaTranslation_def]);
 
-val NLimplementsSequent = store_thm ("NLimplementsSequent",
-  ``implements NL NL_Sequent``,
-    RW_TAC bool_ss [NL_Sequent_def, implements_def]);
+(* Non-associative extension, an empty relation actually *)
+val NL_Sequent_def = Define `
+   (NL_Sequent :'a gentzen_extension) = EMPTY_REL`;
 
 (* NLP Sequent extension *)
-val NLP_Sequent_def = Define `NLP_Sequent A B = NLP (deltaTranslation A) (deltaTranslation B)`;
+val (NLP_Sequent_rules, NLP_Sequent_ind, NLP_Sequent_cases) = Hol_reln `
+    (!A B. NLP_Sequent (Comma A B) (Comma B A))`;
 
-val NLPimplementsSequent = store_thm ("NLPimplementsSequent",
-  ``implements NLP NLP_Sequent``,
-    RW_TAC bool_ss [NLP_Sequent_def, implements_def]);
-
-val NLP_Intro = store_thm ("NLP_Intro", ``!A B. NLP_Sequent (Comma A B) (Comma B A)``,
-    RW_TAC bool_ss [deltaTranslation_def, NLP_Sequent_def, NLP_rules]);
+val NLP_Intro = save_thm ("NLP_Intro", NLP_Sequent_rules);
 
 (* L Sequent extension, the Full Lambek Sequent Calculus extension *)
-val L_Sequent_def = Define `L_Sequent A B = L (deltaTranslation A) (deltaTranslation B)`;
+val (L_Sequent_rules, L_Sequent_ind, L_Sequent_cases) = Hol_reln `
+    (!A B C. L_Sequent (Comma A (Comma B C)) (Comma (Comma A B) C)) /\
+    (!A B C. L_Sequent (Comma (Comma A B) C) (Comma A (Comma B C)))`;
 
-val LimplementsSequent = store_thm ("LimplementsSequent",
-  ``implements L L_Sequent``,
-    RW_TAC bool_ss [L_Sequent_def, implements_def]);
-
-(* two important L_Intro rules now become theorems *)
 local
-  val t = RW_TAC bool_ss [deltaTranslation_def, L_Sequent_def, L_rules]
+    val list = CONJUNCTS L_Sequent_rules
 in
-  val L_Intro_lr = store_thm ("L_Intro_lr",
-    ``!A B C. L_Sequent (Comma A (Comma B C)) (Comma (Comma A B) C)``, t)
-  and L_Intro_rl = store_thm ("L_Intro_rl",
-    ``!A B C. L_Sequent (Comma (Comma A B) C) (Comma A (Comma B C))``, t)
+    val L_Intro_lr = save_thm ("L_Intro_lr", List.nth (list, 0))
+    and L_Intro_rl = save_thm ("L_Intro_rl", List.nth (list, 1))
 end;
 
-val LP_Sequent_def = Define `LP_Sequent = add_extension NLP_Sequent L_Sequent`;
+val LP_Sequent_def = Define `
+    LP_Sequent = add_extension NLP_Sequent L_Sequent`;
+
+val NLP_Sequent_LP_Sequent = store_thm (
+   "NLP_Sequent_LP_Sequent", ``extends NLP_Sequent LP_Sequent``,
+    REWRITE_TAC [LP_Sequent_def, add_extend_l]);
+
+val L_Sequent_LP_Sequent = store_thm (
+   "L_Sequent_LP_Sequent", ``extends L_Sequent LP_Sequent``,
+    REWRITE_TAC [LP_Sequent_def, add_extend_r]);
 
 val LPextendsL = store_thm ("LPextendsL",
   ``!E. extends LP_Sequent E ==> extends L_Sequent E``,
-    RW_TAC bool_ss [LP_Sequent_def, extends_def, RSUBSET, RUNION]);
+    RW_TAC bool_ss [LP_Sequent_def, RSUBSET, RUNION]);
 
 val LPextendsNLP = store_thm ("LPextendsNLP",
   ``!E. extends LP_Sequent E ==> extends NLP_Sequent E``,
-    RW_TAC bool_ss [LP_Sequent_def, extends_def, RSUBSET, RUNION]);
+    RW_TAC bool_ss [LP_Sequent_def, RSUBSET, RUNION]);
 
-val LPimplementsSequent = store_thm ("LPimplementsSequent",
-  ``implements LP LP_Sequent``,
-    REWRITE_TAC [implements_def]
- >> RW_TAC bool_ss [LP_def, LP_Sequent_def]
- >> REWRITE_TAC [RUNION]
- >> RW_TAC bool_ss [NLP_Sequent_def, L_Sequent_def]);
-
-(*** Module: ReplaceProp ***)
+(******************************************************************************)
+(*                                                                            *)
+(*                            Module: ReplaceProp                             *)
+(*                                                                            *)
+(******************************************************************************)
 
 (* The `replace` operator has the type ('a ReplaceProp) *)
 val _ = type_abbrev ("ReplaceProp", ``:'a Term -> 'a Term -> 'a Term -> 'a Term -> bool``);
@@ -374,7 +460,7 @@ val _ = type_abbrev ("ReplaceProp", ``:'a Term -> 'a Term -> 'a Term -> 'a Term 
    then Gamma' results from replacing a distinguished occurrence of the subterm Delta in
    the term Gamma by Delta' *)
 
-val (replace_rules, replace_ind, _) = Hol_reln `
+val (replace_rules, replace_ind, replace_cases) = Hol_reln `
     (!F1 F2. replace F1 F2 F1 F2) /\					(* replaceRoot *)
     (!Gamma1 Gamma2 Delta F1 F2.
      replace Gamma1 Gamma2 F1 F2 ==>
@@ -383,7 +469,13 @@ val (replace_rules, replace_ind, _) = Hol_reln `
      replace Gamma1 Gamma2 F1 F2 ==>
      replace (Comma Delta Gamma1) (Comma Delta Gamma2) F1 F2)`;		(* replaceRight *)
 
-val [replaceRoot, replaceLeft, replaceRight] = CONJ_LIST 3 replace_rules;
+local
+    val list = CONJUNCTS replace_rules
+in
+    val replaceRoot  = save_thm ("replaceRoot[simp]",  List.nth (list, 0))
+    and replaceLeft  = save_thm ("replaceLeft",  List.nth (list, 1))
+    and replaceRight = save_thm ("replaceRight", List.nth (list, 2))
+end;
 
 (* Definition of `replaceCommaDot` such that when ``replaceCommaDot Gamma Gamma'``
    then Gamma' is the result of replacing a number of commas in Gamma by the connector dot.
@@ -391,17 +483,15 @@ val [replaceRoot, replaceLeft, replaceRight] = CONJ_LIST 3 replace_rules;
    Example: ``!A B. replaceCommaDot (A , (A , B)) (A , (A . B)))`` where in this case only
    one occurrence of comma is replaced by a dot. *)
 
-val (replaceCommaDot1_rules, _ , replaceCommaDot1_cases) = Hol_reln `
-    (!T1 T2 A B.
-     replace T1 T2 (Comma (OneForm A) (OneForm B)) (OneForm (Dot A B)) ==>
-     replaceCommaDot1 T1 T2)`;
+val (replaceCommaDot1_rules, replaceCommaDot1_ind, replaceCommaDot1_cases) = Hol_reln `
+    (!T1 T2 A B. replace T1 T2 (Comma (OneForm A) (OneForm B)) (OneForm (Dot A B))
+	     ==> replaceCommaDot1 T1 T2)`;
 
 val replaceCommaDot_def = Define `replaceCommaDot = RTC replaceCommaDot1`;
 
 val replaceCommaDot_rule = store_thm ("replaceCommaDot_rule",
-  ``!T1 T2 A B.
-    replace T1 T2 (Comma (OneForm A) (OneForm B)) (OneForm (Dot A B)) ==>
-    replaceCommaDot T1 T2``,
+  ``!T1 T2 A B. replace T1 T2 (Comma (OneForm A) (OneForm B)) (OneForm (Dot A B))
+	    ==> replaceCommaDot T1 T2``,
     PROVE_TAC [replaceCommaDot_def, replaceCommaDot1_rules, RTC_SINGLE]);
 
 val replaceTransitive = store_thm ("replaceTransitive", ``transitive replaceCommaDot``,
@@ -412,7 +502,7 @@ val replaceTransitive' = store_thm ("replaceTransitive'",
   ``!T1 T2 T3. replaceCommaDot T1 T2 /\ replaceCommaDot T2 T3 ==> replaceCommaDot T1 T3``,
     PROVE_TAC [replaceTransitive, transitive_def]);
 
-val noReplace = store_thm ("noReplace", ``!T. replaceCommaDot T T``,
+val noReplace = store_thm ("noReplace[simp]", ``!T. replaceCommaDot T T``,
     PROVE_TAC [replaceCommaDot_def, RTC_REFLEXIVE, reflexive_def]);
 
 local
@@ -420,28 +510,26 @@ local
 		     transitive_def, RTC_SINGLE]
 in
   val replaceOneComma = store_thm ("replaceOneComma",
-    ``!T1 T2 T3 A B.
-      replaceCommaDot T1 T2 /\
-      replace T2 T3 (Comma (OneForm A) (OneForm B)) (OneForm (Dot A B))
-      ==> replaceCommaDot T1 T3``, t)
+    ``!T1 T2 T3 A B. replaceCommaDot T1 T2 /\
+		     replace T2 T3 (Comma (OneForm A) (OneForm B)) (OneForm (Dot A B))
+		 ==> replaceCommaDot T1 T3``, t)
 
   and replaceOneComma' = store_thm ("replaceOneComma'",
-    ``!T1 T2 T3 A B.
-      replace T1 T2 (Comma (OneForm A) (OneForm B)) (OneForm (Dot A B)) /\
-      replaceCommaDot T2 T3
-      ==> replaceCommaDot T1 T3``, t);
+    ``!T1 T2 T3 A B. replace T1 T2 (Comma (OneForm A) (OneForm B)) (OneForm (Dot A B)) /\
+		     replaceCommaDot T2 T3
+		 ==> replaceCommaDot T1 T3``, t);
 
-  val replaceCommaDot_rules = LIST_CONJ [noReplace, replaceCommaDot_rule,
-					 replaceOneComma, replaceOneComma']
+  val replaceCommaDot_rules = save_thm (
+     "replaceCommaDot_rules", LIST_CONJ [noReplace, replaceCommaDot_rule,
+					 replaceOneComma, replaceOneComma'])
 end;
 
 (* An induction theorem for RTC replaceCommaDot1, similar to those generated by Hol_reln *)
 val replaceCommaDot_ind = store_thm ("replaceCommaDot_ind",
   ``!(P:'a gentzen_extension).
-     (!x. P x x) /\
-     (!x y z A B.
-       replace x y (Comma (OneForm A) (OneForm B)) (OneForm (Dot A B)) /\ P y z ==> P x z)
-     ==> (!x y. replaceCommaDot x y ==> P x y)``,
+	(!x. P x x) /\
+	(!x y z A B. replace x y (Comma (OneForm A) (OneForm B)) (OneForm (Dot A B)) /\ P y z ==> P x z)
+    ==> (!x y. replaceCommaDot x y ==> P x y)``,
  (* The idea is to use RTC_INDUCT thm to prove induct theorems for RTCs *)
     REWRITE_TAC [replaceCommaDot_def]
  >> GEN_TAC   (* remove outer !P *)
@@ -450,19 +538,21 @@ val replaceCommaDot_ind = store_thm ("replaceCommaDot_ind",
  >> PROVE_TAC [replaceCommaDot1_cases]);
 
 local
-  val t = GEN_TAC (* prepare for higher order matching and induction *)
-	  >> HO_MATCH_MP_TAC replaceCommaDot_ind
-	  >> PROVE_TAC [replace_rules, replaceCommaDot_rules]
+  val t = GEN_TAC \\ (* prepare for higher order matching and induction *)
+	  HO_MATCH_MP_TAC replaceCommaDot_ind \\
+	  PROVE_TAC [replace_rules, replaceCommaDot_rules]
 in
   val replaceMonoRight = store_thm ("replaceMonoRight",
-    ``!T3 T1 T2. replaceCommaDot T1 T2 ==> replaceCommaDot (Comma T1 T3) (Comma T2 T3)``, t)
+    ``!T3 T1 T2. replaceCommaDot T1 T2
+	     ==> replaceCommaDot (Comma T1 T3) (Comma T2 T3)``, t)
   and replaceMonoLeft = store_thm ("replaceMonoLeft",
-    ``!T3 T1 T2. replaceCommaDot T1 T2 ==> replaceCommaDot (Comma T3 T1) (Comma T3 T2)``, t)
+    ``!T3 T1 T2. replaceCommaDot T1 T2
+	     ==> replaceCommaDot (Comma T3 T1) (Comma T3 T2)``, t)
 end;
 
 val replaceMono = store_thm ("replaceMono",
-  ``!T1 T2 T3 T4. replaceCommaDot T1 T2 /\ replaceCommaDot T3 T4 ==>
-		  replaceCommaDot (Comma T1 T3) (Comma T2 T4)``,
+  ``!T1 T2 T3 T4. replaceCommaDot T1 T2 /\ replaceCommaDot T3 T4
+	      ==> replaceCommaDot (Comma T1 T3) (Comma T2 T4)``,
     REPEAT STRIP_TAC
  >> MATCH_MP_TAC replaceTransitive'
  >> EXISTS_TAC ``Comma T2 T3``
@@ -471,195 +561,280 @@ val replaceMono = store_thm ("replaceMono",
 val replaceTranslation = store_thm ("replaceTranslation",
   ``!T. replaceCommaDot T (OneForm (deltaTranslation T))``,
     Induct
- >| [ PROVE_TAC [deltaTranslation_def, noReplace], (* base case *)
-      REWRITE_TAC [deltaTranslation_def]         (* induct case *)
-   >> MATCH_MP_TAC replaceTransitive'
-   >> EXISTS_TAC ``Comma (OneForm (deltaTranslation T')) (OneForm (deltaTranslation T''))``
-   >> PROVE_TAC [replaceOneComma, noReplace, replaceRoot, replaceMono] ]);
+ >- PROVE_TAC [deltaTranslation_def, noReplace] (* base case *)
+ >> REWRITE_TAC [deltaTranslation_def]        (* induct case *)
+ >> MATCH_MP_TAC replaceTransitive'
+ >> EXISTS_TAC ``Comma (OneForm (deltaTranslation T')) (OneForm (deltaTranslation T''))``
+ >> PROVE_TAC [replaceOneComma, noReplace, replaceRoot, replaceMono]);
 
-(* TODO / remain theorems: replace_inv1, replace_inv2, doubleReplace, replaceSameP, replaceTrans *)
+val replace_inv1 = store_thm ("replace_inv1",
+  ``!Gamma' Delta X C.
+     replace (OneForm C) Gamma' (OneForm X) Delta ==> (Gamma' = Delta) /\ (X = C)``,
+    REPEAT GEN_TAC
+ >> ONCE_REWRITE_TAC [replace_cases] \\
+ REPEAT STRIP_TAC
+ >- ASM_REWRITE_TAC []
+ >- PROVE_TAC [Term_11]
+ >> PROVE_TAC [Term_distinct]);
 
-(*** Module: NaturalDeduction ***)
+val replace_inv2 = store_thm ("replace_inv2",
+  ``!Gamma1 Gamma2 Gamma' Delta X.
+     replace (Comma Gamma1 Gamma2) Gamma' (OneForm X) Delta ==>
+     (?G. (Gamma' = Comma G Gamma2) /\ replace Gamma1 G (OneForm X) Delta) \/
+     (?G. (Gamma' = Comma Gamma1 G) /\ replace Gamma2 G (OneForm X) Delta)``,
+    REPEAT STRIP_TAC
+ >> POP_ASSUM (MP_TAC o (ONCE_REWRITE_RULE [replace_cases]))
+ >> REPEAT STRIP_TAC
+ >- PROVE_TAC [Term_distinct]
+ >| [ `(Gamma1 = Gamma1') /\ (Gamma2 = Delta')` by PROVE_TAC [Term_11] \\
+      ASM_REWRITE_TAC [] \\
+      MATCH_MP_TAC OR_INTRO_THM1 \\
+      Q.EXISTS_TAC `Gamma2'` \\
+      ASM_REWRITE_TAC [] ,
+      `(Gamma1 = Delta') /\ (Gamma2 = Gamma1')` by PROVE_TAC [Term_11] \\
+      ASM_REWRITE_TAC [] \\
+      MATCH_MP_TAC OR_INTRO_THM2 \\
+      Q.EXISTS_TAC `Gamma2'` \\
+      ASM_REWRITE_TAC [] ]);
 
-val (natDed_rules, _ , _) = Hol_reln `
-    (!(E:'a gentzen_extension) A . natDed E (OneForm A) A) /\			(* NatAxiom *)
-    (!E Gamma A B.								(* SlashIntro *)
-      natDed E (Comma Gamma (OneForm B)) A ==> natDed E Gamma (Slash A B)) /\
-    (!E Gamma A B.								(* BackslashIntro *)
-      natDed E (Comma (OneForm B) Gamma) A ==> natDed E Gamma (Backslash B A)) /\
-    (!E Gamma Delta A B.							(* DotIntro *)
-      natDed E Gamma A /\ natDed E Delta B ==> natDed E (Comma Gamma Delta) (Dot A B)) /\
-    (!E Gamma Delta A B.							(* SlashElim *)
-      natDed E Gamma (Slash A B) /\ natDed E Delta B ==> natDed E (Comma Gamma Delta) A) /\
-    (!E Gamma Delta A B.						 	(* BackslashElim *)
-      natDed E Gamma B /\ natDed E Delta (Backslash B A) ==> natDed E (Comma Gamma Delta) A) /\
-    (!E Gamma Gamma' Delta A B C.						(* DotElim *)
+val doubleReplace = store_thm ("doubleReplace",
+  ``!Gamma Gamma' T1 T2.
+     replace Gamma Gamma' T1 T2 ==>
+     !Gamma2 A T3. replace Gamma' Gamma2 (OneForm A) T3 ==>
+	      (?G. replace Gamma G (OneForm A) T3 /\ replace G Gamma2 T1 T2) \/
+	      (?G. replace T2 G (OneForm A) T3 /\ replace Gamma Gamma2 T1 G)``,
+    Induct_on `replace`
+ >> REPEAT STRIP_TAC (* 3 sub-goals here *)
+ >| [ (* goal 1 (of 3) *)
+      DISJ2_TAC \\
+      Q.EXISTS_TAC `Gamma2` >> ASM_REWRITE_TAC [replaceRoot],
+      (* goal 2 (of 3) *)
+      POP_ASSUM (MP_TAC o (MATCH_MP replace_inv2)) \\
+      REPEAT STRIP_TAC >| (* 2 sub-goals here *)
+      [ (* goal 2.1 (of 2) *)
+        ASM_REWRITE_TAC [] >> RES_TAC >| (* 2 sub-goals here *)
+        [ (* goal 2.1.1 (of 2) *)
+          DISJ1_TAC \\
+          EXISTS_TAC ``(Comma G' Delta)`` \\
+          CONJ_TAC >| (* 2 sub-goals here *)
+          [ (* goal 2.1.1.1 (of 2) *)
+            MATCH_MP_TAC replaceLeft >> ASM_REWRITE_TAC [],
+            (* goal 2.1.1.2 (of 2) *)
+            MATCH_MP_TAC replaceLeft >> ASM_REWRITE_TAC [] ],
+          (* goal 2.1.2 (of 2) *)
+          DISJ2_TAC \\
+          Q.EXISTS_TAC `G'` \\
+          CONJ_TAC >- ASM_REWRITE_TAC [] \\
+          MATCH_MP_TAC replaceLeft >> ASM_REWRITE_TAC [] ],
+        (* goal 2.2 (of 2) *)
+        ASM_REWRITE_TAC [] \\
+        DISJ1_TAC \\
+        EXISTS_TAC ``(Comma Gamma G)`` \\
+        CONJ_TAC >| (* 2 sub-goals here *)
+        [ (* goal 2.2.1 (of 2) *)
+          MATCH_MP_TAC replaceRight >> ASM_REWRITE_TAC [],
+          (* goal 2.2.2 (of 2) *)
+          MATCH_MP_TAC replaceLeft >> ASM_REWRITE_TAC [] ] ],
+      (* goal 3 (of 3) *)
+      POP_ASSUM (MP_TAC o (MATCH_MP replace_inv2)) \\
+      REPEAT STRIP_TAC >| (* 2 sub-goals here *)
+      [ (* goal 3.1 (of 2) *)
+        ASM_REWRITE_TAC [] \\
+        DISJ1_TAC \\
+        EXISTS_TAC ``(Comma G Gamma)`` \\
+        CONJ_TAC >| (* 2 sub-goals here *)
+        [ (* goal 3.1.1 (of 2) *)
+          MATCH_MP_TAC replaceLeft >> ASM_REWRITE_TAC [],
+          (* goal 3.1.2 (of 2) *)
+          MATCH_MP_TAC replaceRight >> ASM_REWRITE_TAC [] ],
+        (* goal 3.2 (of 2) *)
+        ASM_REWRITE_TAC [] >> RES_TAC >| (* 2 sub-goals here *)
+        [ (* goal 3.2.1 (of 2) *)
+          DISJ1_TAC \\
+          EXISTS_TAC ``(Comma Delta G')`` \\
+          CONJ_TAC >| (* 2 sub-goals here *)
+          [ (* goal 3.2.1.1 (of 2) *)
+            MATCH_MP_TAC replaceRight >> ASM_REWRITE_TAC [],
+            (* goal 3.2.1.2 (of 2) *)
+            MATCH_MP_TAC replaceRight >> ASM_REWRITE_TAC [] ],
+          (* goal 3.2.2 (of 2) *)
+          DISJ2_TAC \\
+          Q.EXISTS_TAC `G'` \\
+          CONJ_TAC >- ASM_REWRITE_TAC [] \\
+          MATCH_MP_TAC replaceRight >> ASM_REWRITE_TAC [] ] ] ]);
+
+val replaceSameP = store_thm ("replaceSameP",
+  ``!T1 T2 T3 T4. replace T1 T2 T3 T4 ==>
+		  !G. ?G'. replace T1 G' T3 G /\ replace G' T2 G T4``,
+    Induct_on `replace`
+ >> REPEAT STRIP_TAC
+ >| [ Q.EXISTS_TAC `G` >> REWRITE_TAC [replaceRoot],
+      POP_ASSUM (ASSUME_TAC o (Q.SPEC `G`))
+   >> POP_ASSUM CHOOSE_TAC
+   >> EXISTS_TAC ``(Comma G' Delta)``
+   >> RW_TAC bool_ss [replaceLeft],
+      POP_ASSUM (ASSUME_TAC o (Q.SPEC `G`))
+   >> POP_ASSUM CHOOSE_TAC
+   >> EXISTS_TAC ``(Comma Delta G')``
+   >> RW_TAC bool_ss [replaceRight] ]);
+
+val replaceTrans = store_thm ("replaceTrans",
+  ``!T5 T6 T1 T2 T3 T4.
+     replace T1 T2 T3 T4 ==> replace T3 T4 T5 T6 ==> replace T1 T2 T5 T6``,
+    NTAC 2 GEN_TAC
+ >> Induct_on `replace`
+ >> REPEAT STRIP_TAC
+ >| [ PROVE_TAC [replaceLeft],
+      PROVE_TAC [replaceRight] ]);
+
+(* easier for MATCH_MP_TAC *)
+val replaceTrans' = store_thm ("replaceTrans'",
+  ``!T5 T6 T1 T2 T3 T4.
+     replace T1 T2 T3 T4 /\ replace T3 T4 T5 T6 ==> replace T1 T2 T5 T6``,
+    PROVE_TAC [replaceTrans]);
+
+(******************************************************************************)
+(*                                                                            *)
+(*                         Module: NaturalDeduction                           *)
+(*                                                                            *)
+(******************************************************************************)
+
+val (natDed_rules, natDed_ind, natDed_cases) = Hol_reln `
+    (!(E:'a gentzen_extension) A.				(* NatAxiom *)
+      natDed E (OneForm A) A) /\
+    (!E Gamma A B.						(* SlashIntro *)
+      natDed E (Comma Gamma (OneForm B)) A ==>
+      natDed E Gamma (Slash A B)) /\
+    (!E Gamma A B.						(* BackslashIntro *)
+      natDed E (Comma (OneForm B) Gamma) A ==>
+      natDed E Gamma (Backslash B A)) /\
+    (!E Gamma Delta A B.					(* DotIntro *)
+      natDed E Gamma A /\ natDed E Delta B ==>
+      natDed E (Comma Gamma Delta) (Dot A B)) /\
+    (!E Gamma Delta A B.					(* SlashElim *)
+      natDed E Gamma (Slash A B) /\ natDed E Delta B ==>
+      natDed E (Comma Gamma Delta) A) /\
+    (!E Gamma Delta A B.				 	(* BackslashElim *)
+      natDed E Gamma B /\ natDed E Delta (Backslash B A) ==>
+      natDed E (Comma Gamma Delta) A) /\
+    (!E Gamma Gamma' Delta A B C.				(* DotElim *)
       replace Gamma Gamma' (Comma (OneForm A) (OneForm B)) Delta /\
-      natDed E Delta (Dot A B) /\ natDed E Gamma C ==> natDed E Gamma' C) /\
-    (!(E:'a gentzen_extension) C Gamma Gamma' Delta Delta'.			(* NatExt *)
+      natDed E Delta (Dot A B) /\ natDed E Gamma C ==>
+      natDed E Gamma' C) /\
+    (!(E:'a gentzen_extension) C Gamma Gamma' Delta Delta'.	(* NatExt *)
       replace Gamma Gamma' Delta Delta' /\ E Delta Delta' /\
       natDed E Gamma C ==> natDed E Gamma' C)`;
 
-val [NatAxiom, SlashIntro, BackslashIntro, DotIntro, SlashElim, BackslashElim, DotElim, NatExt] =
-    (CONJ_LIST 8 natDed_rules);
+local
+    val list = CONJUNCTS natDed_rules
+in
+    val NatAxiom       = save_thm ("NatAxiom[simp]", List.nth (list, 0))
+    and SlashIntro     = save_thm ("SlashIntro",     List.nth (list, 1))
+    and BackslashIntro = save_thm ("BackslashIntro", List.nth (list, 2))
+    and DotIntro       = save_thm ("DotIntro",       List.nth (list, 3))
+    and SlashElim      = save_thm ("SlashElim",      List.nth (list, 4))
+    and BackslashElim  = save_thm ("BackslashElim",  List.nth (list, 5))
+    and DotElim        = save_thm ("DotElim",        List.nth (list, 6))
+    and NatExt         = save_thm ("NatExt",         List.nth (list, 7))
+end;
 
-(* Alternative definition, above natDed_rules then become deriable theorems from Arrow_rules
-val natDed_def = Define `
-    natDed E Gamma A = (!X. implements X E ==> Arrow X (deltaTranslation Gamma) A)`;
-
-val NatAxiom = store_thm ("NatAxiom", ``!E A. natDed E (OneForm A) A``,
-    REWRITE_TAC [natDed_def, deltaTranslation_def]
- >> REPEAT STRIP_TAC
- >> REWRITE_TAC [one]);
-
-val SlashIntro = store_thm ("SlashIntro",
-  ``(!E Gamma A B. natDed E (Comma Gamma (OneForm B)) A ==> natDed E Gamma (Slash A B))``,
-    REWRITE_TAC [natDed_def, deltaTranslation_def]
- >> PROVE_TAC [beta]);
-
-val BackslashIntro = store_thm ("BackslashIntro",
-  ``(!E Gamma A B. natDed E (Comma (OneForm B) Gamma) A ==> natDed E Gamma (Backslash B A))``,
-    REWRITE_TAC [natDed_def, deltaTranslation_def]
- >> PROVE_TAC [gamma]);
-
-(* this is rule (5) in Lambek (1958), from arrow rule (L_m) *)
-val DotIntro = store_thm ("DotIntro'",
-  ``!E Gamma Delta A B. natDed E Gamma A /\ natDed E Delta B
-		    ==> natDed E (Comma Gamma Delta) (Dot A B)``,
-    RW_TAC bool_ss [natDed_def, deltaTranslation_def]
- >> PROVE_TAC [Arrow_rules]);
-
-val SlashElim = store_thm ("SlashElim",
-  ``!E Gamma Delta A B. natDed E Gamma (Slash A B) /\ natDed E Delta B
-		    ==> natDed E (Comma Gamma Delta) A``,
-    RW_TAC bool_ss [natDed_def, deltaTranslation_def]
- >> PROVE_TAC [Arrow_rules]);
-
-val BackslashElim = store_thm ("BackslashElim'",
-  ``!E Gamma Delta A B. natDed E Gamma B /\ natDed E Delta (Backslash B A)
-		    ==> natDed E (Comma Gamma Delta) A``,
-    RW_TAC bool_ss [natDed_def, deltaTranslation_def]
- >> PROVE_TAC [Arrow_rules]);
- *)
-
-val NatAxiomGen = store_thm ("NatAxiomGen", ``!E Gamma. natDed E Gamma (deltaTranslation Gamma)``,
+val NatAxiomGeneralized = store_thm ("NatAxiomGeneralized[simp]",
+  ``!E Gamma. natDed E Gamma (deltaTranslation Gamma)``,
     Induct_on `Gamma:'a Term`
- >| [ PROVE_TAC [deltaTranslation_def, NatAxiom], (* base case *)
-      REWRITE_TAC [deltaTranslation_def]        (* induct case *)
-   >> PROVE_TAC [DotIntro] ]);
-
-(* from GentzenDed.v, induction required, to be used for proving DotElim *)
-val replaceNatDed = store_thm ("replaceNatDed",
-  ``!E Gamma Gamma' Delta Delta'.
-    replace Gamma Gamma' Delta Delta' ==>
-    natDed E Delta' (deltaTranslation Delta) ==>
-    natDed E Gamma' (deltaTranslation Gamma)``,
-    GEN_TAC
- >> HO_MATCH_MP_TAC replace_ind
- >> CONJ_TAC THEN1 RW_TAC bool_ss []
+ >- PROVE_TAC [deltaTranslation_def, NatAxiom]
  >> REWRITE_TAC [deltaTranslation_def]
- >> CONJ_TAC
- >> REPEAT STRIP_TAC
- >> MATCH_MP_TAC DotIntro
- >> RW_TAC bool_ss [NatAxiomGen]);
-
-(* 
-val DotElim = store_thm ("DotElim",
-  ``!E Gamma Gamma' Delta' A B C.
-     replace Gamma Gamma' (Comma (OneForm A) (OneForm B)) Delta' ==>
-     natDed E Delta' (Dot A B) ==>
-     natDed E Gamma C ==>
-     natDed E Gamma' C``,
-    REPEAT STRIP_TAC
- >> `natDed E Gamma' (deltaTranslation Gamma)` by PROVE_TAC [replaceNatDed, deltaTranslation_def]
- >> `natDed E Gamma (deltaTranslation Gamma)` by PROVE_TAC [NatAxiomGen]
- >> PROVE_TAC [natDed_def, Arrow_rules]);
-*)
-
-(* TODO: NatExt should be proved using arrow_plus or nothing ...
-val NatExt = store_thm ("NatExt",
-  ``!E C Gamma Gamma' Delta Delta'.
-    replace Gamma Gamma' Delta Delta' ==> E Delta Delta' ==> natDed E Gamma C ==> natDed E Gamma' C``,
-    NTAC 2 GEN_TAC
- >> HO_MATCH_MP_TAC replace_ind
- >> REPEAT STRIP_TAC (* 3 sub-goals here *)
- >| [ UNDISCH_TAC ``natDed E Gamma C``
-   >> RW_TAC bool_ss [natDed_def] 
-   >> `Arrow X (deltaTranslation Gamma) C` by PROVE_TAC []
-   >> `X (deltaTranslation Gamma) (deltaTranslation Gamma')` by PROVE_TAC [implements_def]
-   >> `Arrow X (deltaTranslation Gamma) (deltaTranslation Gamma')` by PROVE_TAC [arrow_plus]
-   >> PROVE_TAC [Arrow_rules]
-   >> , , ] );
-
-val natDed_rules = LIST_CONJ [NatAxiom, SlashIntro, BackslashIntro, DotIntro,
-			      SlashElim, BackslashElim, DotElim]; (* NatExt *)
- *)
+ >> PROVE_TAC [DotIntro]);
 
 val DotElimGeneralized = store_thm ("DotElimGeneralized",
-  ``!E C Gamma Gamma'. replaceCommaDot Gamma Gamma' ==> natDed E Gamma C ==> natDed E Gamma' C``,
+  ``!E C Gamma Gamma'. replaceCommaDot Gamma Gamma'
+		   ==> natDed E Gamma C ==> natDed E Gamma' C``,
     NTAC 2 GEN_TAC
  >> HO_MATCH_MP_TAC replaceCommaDot_ind
  >> REPEAT STRIP_TAC
- >> `natDed E (OneForm (Dot A B)) (Dot A B)` by PROVE_TAC [NatAxiomGen, deltaTranslation_def]
+ >> `natDed E (OneForm (Dot A B)) (Dot A B)` by PROVE_TAC [NatAxiomGeneralized, deltaTranslation_def]
  >> `natDed E Gamma' C` by PROVE_TAC [DotElim]
  >> RW_TAC bool_ss []);
 
-val TermToFormDed = store_thm ("TermToFormDed",
+val NatTermToForm = store_thm ("NatTermToForm",
   ``!E Gamma C. natDed E Gamma C ==> natDed E (OneForm (deltaTranslation Gamma)) C``,
     REPEAT STRIP_TAC
  >> PROVE_TAC [DotElimGeneralized, replaceTranslation]);
 
-(*** Module: Sequent Calculus ***)
+val NatExtSimpl = store_thm (
+   "NatExtSimpl", ``!E Gamma Gamma' C. E Gamma Gamma' /\ natDed E Gamma C ==> natDed E Gamma' C``,
+    REPEAT STRIP_TAC
+ >> `replace Gamma Gamma' Gamma Gamma'` by REWRITE_TAC [replaceRoot]
+ >> IMP_RES_TAC NatExt);
 
-(* NOTE: it's a little meaningless to try to derive these rules from Arrow rules or NatDed rules,
-   because after all the CutRule cannot be proved inside these systems (however, we're going to
-   prove any gentzenSequent proof has a corresponding Cut-free proof, thus CutRule can be eliminated *)
+(******************************************************************************)
+(*                                                                            *)
+(*                        Module: Sequent Calculus                            *)
+(*                                                                            *)
+(******************************************************************************)
 
-(* gentzen presentation using sequents: sequent is a pair (Gamma, A) where: *)
-val (gentzenSequent_rules, gentzenSequent_ind, _) = Hol_reln `
-    (!(E:'a gentzen_extension) A. gentzenSequent E (OneForm A) A) /\	(* SeqAxiom = NatAxiom *)
-    (!E Gamma A B.							(* RightSlash = SlashIntro *)
+(* gentzen presentation using sequents. *)
+val (gentzenSequent_rules, gentzenSequent_ind, gentzenSequent_cases) = Hol_reln `
+    (!(E:'a gentzen_extension) A.				(* SeqAxiom = NatAxiom *)
+      gentzenSequent E (OneForm A) A) /\
+    (!E Gamma A B.						(* RightSlash = SlashIntro *)
       gentzenSequent E (Comma Gamma (OneForm B)) A ==>
       gentzenSequent E Gamma (Slash A B)) /\
-    (!E Gamma A B.							(* RightBackslash = BackslashIntro *)
+    (!E Gamma A B.						(* RightBackslash = BackslashIntro *)
       gentzenSequent E (Comma (OneForm B) Gamma) A ==>
       gentzenSequent E Gamma (Backslash B A)) /\
-    (!E Gamma Delta A B.						(* RightDot = DotIntro *)
-      gentzenSequent E Gamma A /\ gentzenSequent E Delta B
-      ==> gentzenSequent E (Comma Gamma Delta) (Dot A B)) /\
-    (!E Gamma Gamma' Delta A B C.					(* LeftSlash != SlashElim *)
+    (!E Gamma Delta A B.					(* RightDot = DotIntro *)
+      gentzenSequent E Gamma A /\ gentzenSequent E Delta B ==>
+      gentzenSequent E (Comma Gamma Delta) (Dot A B)) /\
+
+    (* Delta |- B /\ Gamma[A] |- C ==> Gamma[A / B, Delta] |- C  *)
+    (!E Gamma Gamma' Delta A B C.				(* LeftSlash *)
       replace Gamma Gamma' (OneForm A) (Comma (OneForm (Slash A B)) Delta) /\
-      gentzenSequent E Delta B /\ gentzenSequent E Gamma C
-      ==> gentzenSequent E Gamma' C) /\
-    (!E Gamma Gamma' Delta A B C.					(* LeftBackslash != BackslashElim *)
+      gentzenSequent E Delta B /\ gentzenSequent E Gamma C ==>
+      gentzenSequent E Gamma' C) /\
+
+    (* Delta |- B /\ Gamma[A] |- C ==> Gamma[Delta, B \ A] |- C *)
+    (!E Gamma Gamma' Delta A B C.				(* LeftBackslash *)
       replace Gamma Gamma' (OneForm A) (Comma Delta (OneForm (Backslash B A))) /\
-      gentzenSequent E Delta B /\ gentzenSequent E Gamma C
-      ==> gentzenSequent E Gamma' C) /\
-    (!E Gamma Gamma' A B C.						(* LeftDot != DotElim *)
+      gentzenSequent E Delta B /\ gentzenSequent E Gamma C ==>
+      gentzenSequent E Gamma' C) /\
+
+    (* Gamma[A, B] |- C ==> Gamma[A * B] |- C *)
+    (!E Gamma Gamma' A B C.					(* LeftDot *)
       replace Gamma Gamma' (Comma (OneForm A) (OneForm B)) (OneForm (Dot A B)) /\
-      gentzenSequent E Gamma C
-      ==> gentzenSequent E Gamma' C) /\
-    (!E Delta Gamma Gamma' A C.						(* CutRule is new *)
+      gentzenSequent E Gamma C ==>
+      gentzenSequent E Gamma' C) /\
+
+    (* Delta |- A /\ Gamma[A] |- C ==> Gamma[Delta] |- C *)
+    (!E Delta Gamma Gamma' A C.					(* CutRule *)
       replace Gamma Gamma' (OneForm A) Delta /\
-      gentzenSequent E Delta A /\ gentzenSequent E Gamma C
-      ==> gentzenSequent E Gamma' C) /\
-    (!(E:'a gentzen_extension) Gamma Gamma' Delta Delta' C.		(* SequentExtension = NatExt *)
-      replace Gamma Gamma' Delta Delta' /\ E Delta Delta' /\ gentzenSequent E Gamma C
-      ==> gentzenSequent E Gamma' C)`;
+      gentzenSequent E Delta A /\ gentzenSequent E Gamma C ==>
+      gentzenSequent E Gamma' C) /\
 
-val [SeqAxiom, RightSlash, RightBackslash, RightDot, LeftSlash, LeftBackslash, LeftDot,
-     CutRule, SequentExtension] = CONJ_LIST 9 gentzenSequent_rules;
+    (* E Delta Delta' /\ Gamma[Delta] |- C ==> Gamma[Delta'] |- C *)
+    (!(E:'a gentzen_extension) Gamma Gamma' Delta Delta' C.	(* SeqExt = NatExt *)
+      replace Gamma Gamma' Delta Delta' /\ E Delta Delta' /\
+      gentzenSequent E Gamma C ==> gentzenSequent E Gamma' C)`;
 
-(* NOTE: deltaTranslation connects two operators Dot (in Forms) and Comma (in Terms).
-         the theorem SeqAxiomGen seems essential for proving some foundamental theorems about
-         Lambek calculu in gentzen's Sequent Calculus form. This made me think that, the above
-         gentzenSequent_rules shouldn't be primitive, at least not all! *)
+local
+    val list = CONJUNCTS gentzenSequent_rules
+in
+    val SeqAxiom       = save_thm ("SeqAxiom[simp]", List.nth (list, 0))
+    and RightSlash     = save_thm ("RightSlash",     List.nth (list, 1))
+    and RightBackslash = save_thm ("RightBackslash", List.nth (list, 2))
+    and RightDot       = save_thm ("RightDot",       List.nth (list, 3))
+    and LeftSlash      = save_thm ("LeftSlash",      List.nth (list, 4))
+    and LeftBackslash  = save_thm ("LeftBackslash",  List.nth (list, 5))
+    and LeftDot        = save_thm ("LeftDot",        List.nth (list, 6))
+    and CutRule        = save_thm ("CutRule",        List.nth (list, 7))
+    and SeqExt         = save_thm ("SeqExt",         List.nth (list, 8))
+end;
 
-val SeqAxiomGen = store_thm ("SeqAxiomGen",
+(* old name: axiomeGeneralisation *)
+val SeqAxiomGeneralized = store_thm ("SeqAxiomGeneralized[simp]",
   ``!E Gamma. gentzenSequent E Gamma (deltaTranslation Gamma)``,
     Induct_on `Gamma:'a Term`
  >| [ PROVE_TAC [deltaTranslation_def, SeqAxiom], (* base case *)
-      REWRITE_TAC [deltaTranslation_def] >>     (* induct case *)
+      REWRITE_TAC [deltaTranslation_def] \\     (* induct case *)
       PROVE_TAC [RightDot] ]);
 
 (* Some derived properties concerning gentzenSequent *)
@@ -681,7 +856,7 @@ val LeftDotGeneralized = store_thm ("LeftDotGeneralized",
  >> REPEAT STRIP_TAC
  >> PROVE_TAC [LeftDot]);
 
-val TermToForm = store_thm ("TermToForm",
+val SeqTermToForm = store_thm ("SeqTermToForm",
   ``!E Gamma C. gentzenSequent E Gamma C
 	    ==> gentzenSequent E (OneForm (deltaTranslation Gamma)) C``,
     REPEAT GEN_TAC
@@ -713,6 +888,13 @@ val DotRightBackslash' = store_thm ("DotRightBackslash'",
 	  ==> gentzenSequent E (OneForm (Dot A B)) C``,
     PROVE_TAC [replace_rules, replaceCommaDot_rules, gentzenSequent_rules]);
 
+val SeqExtSimpl = store_thm (
+   "SeqExtSimpl", ``!E Gamma Gamma' C. E Gamma Gamma' /\ gentzenSequent E Gamma C
+				   ==> gentzenSequent E Gamma' C``,
+    REPEAT STRIP_TAC
+ >> `replace Gamma Gamma' Gamma Gamma'` by REWRITE_TAC [replaceRoot]
+ >> IMP_RES_TAC SeqExt);
+
 (* some definitions concerning extensions *)
 
 val LextensionSimpl = store_thm ("LextensionSimpl",
@@ -720,28 +902,28 @@ val LextensionSimpl = store_thm ("LextensionSimpl",
 		   gentzenSequent E (Comma T1 (Comma T2 T3)) C
 	       ==> gentzenSequent E (Comma (Comma T1 T2) T3) C``,
     REPEAT STRIP_TAC
- >> MATCH_MP_TAC SequentExtension
- >> EXISTS_TAC ``(Comma T1 (Comma T2 T3))``       (* Gamma *)
- >> EXISTS_TAC ``(Comma T1 (Comma T2 T3))``       (* Delta *)
- >> EXISTS_TAC ``(Comma (Comma T1 T2) T3)``       (* Delta' *)
+ >> MATCH_MP_TAC SeqExt
+ >> EXISTS_TAC ``(Comma T1 (Comma T2 T3))``	(* Gamma *)
+ >> EXISTS_TAC ``(Comma T1 (Comma T2 T3))``	(* Delta *)
+ >> EXISTS_TAC ``(Comma (Comma T1 T2) T3)``	(* Delta' *)
  >> REPEAT STRIP_TAC (* 3 sub-goals here *)
- >| [ REWRITE_TAC [replaceRoot],
-      PROVE_TAC [extends_def, RSUBSET, L_Intro_lr],
-      ASM_REWRITE_TAC [] ]);
+ >- REWRITE_TAC [replaceRoot]
+ >- PROVE_TAC [RSUBSET, L_Intro_lr]
+ >> ASM_REWRITE_TAC []);
 
 val LextensionSimpl' = store_thm ("LextensionSimpl'", (* dual theorem of above *)
   ``!E T1 T2 T3 C. extends L_Sequent E /\
 		   gentzenSequent E (Comma (Comma T1 T2) T3) C
 	       ==> gentzenSequent E (Comma T1 (Comma T2 T3)) C``,
     REPEAT STRIP_TAC
- >> MATCH_MP_TAC SequentExtension
- >> EXISTS_TAC ``(Comma (Comma T1 T2) T3)``       (* Gamma *)
- >> EXISTS_TAC ``(Comma (Comma T1 T2) T3)``       (* Delta *)
- >> EXISTS_TAC ``(Comma T1 (Comma T2 T3))``       (* Delta' *)
+ >> MATCH_MP_TAC SeqExt
+ >> EXISTS_TAC ``(Comma (Comma T1 T2) T3)``	(* Gamma *)
+ >> EXISTS_TAC ``(Comma (Comma T1 T2) T3)``	(* Delta *)
+ >> EXISTS_TAC ``(Comma T1 (Comma T2 T3))``	(* Delta' *)
  >> REPEAT STRIP_TAC (* 3 sub-goals here *)
- >| [ REWRITE_TAC [replaceRoot],
-      PROVE_TAC [extends_def, RSUBSET, L_Intro_rl],
-      ASM_REWRITE_TAC [] ]);
+ >- REWRITE_TAC [replaceRoot]
+ >- PROVE_TAC [RSUBSET, L_Intro_rl]
+ >> ASM_REWRITE_TAC []);
 
 val LextensionSimplDot = store_thm ("LextensionSimplDot",
   ``!E A B C D. extends L_Sequent E /\
@@ -754,13 +936,13 @@ val LextensionSimplDot = store_thm ("LextensionSimplDot",
  >> Q.EXISTS_TAC `A`
  >> Q.EXISTS_TAC `B`
  >> STRIP_TAC
- >| [ RW_TAC bool_ss [replaceLeft, replaceRoot],
-      MATCH_MP_TAC LextensionSimpl
-   >> STRIP_TAC
-   >| [ ASM_REWRITE_TAC [],
-	MATCH_MP_TAC CutRuleSimpl
-     >> EXISTS_TAC ``(deltaTranslation (Comma (OneForm A) (Comma (OneForm B) (OneForm C))))``
-     >> RW_TAC bool_ss [SeqAxiomGen, deltaTranslation_def] ] ]);
+ >- RW_TAC bool_ss [replaceLeft, replaceRoot]
+ >> MATCH_MP_TAC LextensionSimpl
+ >> STRIP_TAC
+ >- ASM_REWRITE_TAC []
+ >> MATCH_MP_TAC CutRuleSimpl
+ >> EXISTS_TAC ``(deltaTranslation (Comma (OneForm A) (Comma (OneForm B) (OneForm C))))``
+ >> RW_TAC bool_ss [SeqAxiomGeneralized, deltaTranslation_def]);
 
 val LextensionSimplDot' = store_thm ("LextensionSimplDot'", (* dual theorem of above *)
   ``!E A B C D. extends L_Sequent E /\
@@ -773,27 +955,27 @@ val LextensionSimplDot' = store_thm ("LextensionSimplDot'", (* dual theorem of a
  >> Q.EXISTS_TAC `B`
  >> Q.EXISTS_TAC `C`
  >> STRIP_TAC
- >| [ RW_TAC bool_ss [replaceRight, replaceRoot],
-      MATCH_MP_TAC LextensionSimpl'
-   >> STRIP_TAC
-   >| [ ASM_REWRITE_TAC [],
-	MATCH_MP_TAC CutRuleSimpl
-     >> EXISTS_TAC ``(deltaTranslation (Comma (Comma (OneForm A) (OneForm B)) (OneForm C)))``
-     >> RW_TAC bool_ss [SeqAxiomGen, deltaTranslation_def] ] ]);
+ >- RW_TAC bool_ss [replaceRight, replaceRoot]
+ >> MATCH_MP_TAC LextensionSimpl'
+ >> STRIP_TAC
+ >- ASM_REWRITE_TAC []
+ >> MATCH_MP_TAC CutRuleSimpl
+ >> EXISTS_TAC ``(deltaTranslation (Comma (Comma (OneForm A) (OneForm B)) (OneForm C)))``
+ >> RW_TAC bool_ss [SeqAxiomGeneralized, deltaTranslation_def]);
 
 val NLPextensionSimpl = store_thm ("NLPextensionSimpl",
   ``!E T1 T2 C. extends NLP_Sequent E /\
 		gentzenSequent E (Comma T1 T2) C
 	    ==> gentzenSequent E (Comma T2 T1) C``,
     REPEAT STRIP_TAC
- >> MATCH_MP_TAC SequentExtension
+ >> MATCH_MP_TAC SeqExt
  >> EXISTS_TAC ``(Comma T1 T2)``
  >> EXISTS_TAC ``(Comma T1 T2)``
  >> EXISTS_TAC ``(Comma T2 T1)``
  >> REPEAT STRIP_TAC (* 3 sub-goals here *)
- >| [ REWRITE_TAC [replaceRoot],
-      PROVE_TAC [extends_def, RSUBSET, NLP_Intro],
-      ASM_REWRITE_TAC [] ]);
+ >- REWRITE_TAC [replaceRoot]
+ >- PROVE_TAC [RSUBSET, NLP_Intro]
+ >> ASM_REWRITE_TAC []);
 
 val NLPextensionSimplDot = store_thm ("NLPextensionSimplDot",
   ``!E A B C. extends NLP_Sequent E /\
@@ -803,28 +985,30 @@ val NLPextensionSimplDot = store_thm ("NLPextensionSimplDot",
  >> MATCH_MP_TAC LeftDotSimpl
  >> MATCH_MP_TAC NLPextensionSimpl
  >> STRIP_TAC
- >| [ ASM_REWRITE_TAC [],
-      MATCH_MP_TAC CutRuleSimpl
-   >> EXISTS_TAC ``(deltaTranslation (Comma (OneForm A) (OneForm B)))``
-   >> RW_TAC bool_ss [SeqAxiomGen, deltaTranslation_def] ]);
+ >- ASM_REWRITE_TAC []
+ >> MATCH_MP_TAC CutRuleSimpl
+ >> EXISTS_TAC ``(deltaTranslation (Comma (OneForm A) (OneForm B)))``
+ >> RW_TAC bool_ss [SeqAxiomGeneralized, deltaTranslation_def]);
 
 (* original name: gentzenExtends, see also mono_X *)
 val mono_E = store_thm ("mono_E",
-  ``!E' E Gamma A. gentzenSequent E Gamma A ==> extends E E' ==> gentzenSequent E' Gamma A``,
+  ``!E' E Gamma A. gentzenSequent E Gamma A
+	       ==> extends E E'
+	       ==> gentzenSequent E' Gamma A``,
     GEN_TAC
  >> HO_MATCH_MP_TAC gentzenSequent_ind
- >> REPEAT STRIP_TAC (* 9 goals here, from easy to hard *)
- >| [ REWRITE_TAC [SeqAxiom],
-      RW_TAC bool_ss [RightSlash],
-      RW_TAC bool_ss [RightBackslash],
-      RW_TAC bool_ss [RightDot],
-      PROVE_TAC [LeftSlash],
-      PROVE_TAC [LeftBackslash],
-      PROVE_TAC [LeftDot],
-      PROVE_TAC [CutRule],
-      `E' Delta Delta'` by PROVE_TAC [extends_def, RSUBSET]
-   >> `gentzenSequent E' Gamma A` by RW_TAC bool_ss []
-   >> PROVE_TAC [SequentExtension] ]);
+ >> REPEAT STRIP_TAC (* 9 goals here *)
+ >- REWRITE_TAC [SeqAxiom]
+ >- RW_TAC bool_ss [RightSlash]
+ >- RW_TAC bool_ss [RightBackslash]
+ >- RW_TAC bool_ss [RightDot]
+ >- PROVE_TAC [LeftSlash]
+ >- PROVE_TAC [LeftBackslash]
+ >- PROVE_TAC [LeftDot]
+ >- PROVE_TAC [CutRule]
+ >> `E' Delta Delta'` by PROVE_TAC [RSUBSET]
+ >> `gentzenSequent E' Gamma A` by RW_TAC bool_ss []
+ >> PROVE_TAC [SeqExt]);
 
 (* Some theorems and derived properties
    These definitions can be applied for all gentzen extensions,
@@ -832,11 +1016,17 @@ val mono_E = store_thm ("mono_E",
 
 val application = store_thm ("application",
   ``!E A B. gentzenSequent E (OneForm (Dot (Slash A B) B)) A``,
-    PROVE_TAC [LeftDotSimpl, LeftSlashSimpl, SeqAxiom]);
+    REPEAT STRIP_TAC
+ >> MATCH_MP_TAC LeftDotSimpl
+ >> MATCH_MP_TAC LeftSlashSimpl
+ >> REWRITE_TAC [SeqAxiom]);
 
 val application' = store_thm ("application'",
   ``!E A B. gentzenSequent E (OneForm (Dot B (Backslash B A))) A``,
-    PROVE_TAC [LeftDotSimpl, LeftBackslashSimpl, SeqAxiom]);
+    REPEAT STRIP_TAC
+ >> MATCH_MP_TAC LeftDotSimpl
+ >> MATCH_MP_TAC LeftBackslashSimpl
+ >> REWRITE_TAC [SeqAxiom]);
 
 val RightSlashDot = store_thm ("RightSlashDot",
   ``!E A B C. gentzenSequent E (OneForm (Dot A C)) B
@@ -845,7 +1035,7 @@ val RightSlashDot = store_thm ("RightSlashDot",
  >> MATCH_MP_TAC RightSlash
  >> MATCH_MP_TAC CutRuleSimpl
  >> EXISTS_TAC ``(deltaTranslation (Comma (OneForm A) (OneForm C)))``
- >> RW_TAC bool_ss [SeqAxiomGen, deltaTranslation_def]);
+ >> RW_TAC bool_ss [SeqAxiomGeneralized, deltaTranslation_def]);
 
 val RightBackslashDot = store_thm ("RightBackslashDot",
   ``!E A B C. gentzenSequent E (OneForm (Dot B A)) C
@@ -854,7 +1044,7 @@ val RightBackslashDot = store_thm ("RightBackslashDot",
  >> MATCH_MP_TAC RightBackslash
  >> MATCH_MP_TAC CutRuleSimpl
  >> EXISTS_TAC ``(deltaTranslation (Comma (OneForm B) (OneForm A)))``
- >> RW_TAC bool_ss [SeqAxiomGen, deltaTranslation_def]);
+ >> RW_TAC bool_ss [SeqAxiomGeneralized, deltaTranslation_def]);
 
 val coApplication = store_thm ("coApplication",
   ``!E A B. gentzenSequent E (OneForm A) (Slash (Dot A B) B)``,
@@ -896,8 +1086,8 @@ val antitonicity = store_thm ("antitonicity",
  >> MATCH_MP_TAC CutRuleSimpl
  >> EXISTS_TAC ``(Dot (Slash C B) B)``
  >> STRIP_TAC
- >| [ PROVE_TAC [RightDot, SeqAxiom],
-      REWRITE_TAC [application] ]);
+ >- PROVE_TAC [RightDot, SeqAxiom]
+ >> REWRITE_TAC [application]);
 
 val antitonicity' = store_thm ("antitonicity'",
   ``!E A B C. gentzenSequent E (OneForm A) B
@@ -907,8 +1097,8 @@ val antitonicity' = store_thm ("antitonicity'",
  >> MATCH_MP_TAC CutRuleSimpl
  >> EXISTS_TAC ``(Dot B (Backslash B C))``
  >> STRIP_TAC
- >| [ PROVE_TAC [RightDot, SeqAxiom],
-      REWRITE_TAC [application'] ]);
+ >- PROVE_TAC [RightDot, SeqAxiom]
+ >> REWRITE_TAC [application']);
 
 val lifting = store_thm ("lifting",
   ``!E A B C. gentzenSequent E (OneForm A) (Slash B (Backslash A B))``,
@@ -917,8 +1107,8 @@ val lifting = store_thm ("lifting",
  >> MATCH_MP_TAC CutRuleSimpl
  >> EXISTS_TAC ``(Dot A (Backslash A B))``
  >> STRIP_TAC
- >| [ PROVE_TAC [RightDot, SeqAxiom],
-      REWRITE_TAC [application'] ]);
+ >- PROVE_TAC [RightDot, SeqAxiom]
+ >> REWRITE_TAC [application']);
 
 val lifting' = store_thm ("lifting'",
   ``!E A B C. gentzenSequent E (OneForm A) (Backslash (Slash B A) B)``,
@@ -927,147 +1117,176 @@ val lifting' = store_thm ("lifting'",
  >> MATCH_MP_TAC CutRuleSimpl
  >> EXISTS_TAC ``(Dot (Slash B A) A)``
  >> STRIP_TAC
- >| [ PROVE_TAC [RightDot, SeqAxiom],
-      REWRITE_TAC [application] ]);
+ >- PROVE_TAC [RightDot, SeqAxiom]
+ >> REWRITE_TAC [application]);
 
 (* These definitions can be applied iff associativity is supported by our logical system *)
 
 val mainGeach = store_thm ("mainGeach",
-  ``!E A B C. extends L_Sequent E ==> gentzenSequent E (OneForm (Slash A B))
-						       (Slash (Slash A C) (Slash B C))``,
+  ``!E A B C. extends L_Sequent E
+	  ==> gentzenSequent E (OneForm (Slash A B))
+			       (Slash (Slash A C) (Slash B C))``,
     REPEAT STRIP_TAC
  >> NTAC 2 (MATCH_MP_TAC RightSlash)
  >> MATCH_MP_TAC LextensionSimpl
- >> CONJ_TAC THEN1 (POP_ASSUM ACCEPT_TAC)
+ >> CONJ_TAC
+ >- POP_ASSUM ACCEPT_TAC
  >> MATCH_MP_TAC CutRuleSimpl
  >> EXISTS_TAC ``(Dot (Slash A B) B)``
  >> CONJ_TAC
- >| [ MATCH_MP_TAC RightDot
-   >> CONJ_TAC
-   >| [ REWRITE_TAC [SeqAxiom],
-        MATCH_MP_TAC LeftSlashSimpl >> STRIP_TAC >> REWRITE_TAC [SeqAxiom] ],
+ >| [ MATCH_MP_TAC RightDot \\
+      CONJ_TAC >|
+      [ REWRITE_TAC [SeqAxiom],
+	MATCH_MP_TAC LeftSlashSimpl \\
+	STRIP_TAC \\
+	REWRITE_TAC [SeqAxiom] ],
       REWRITE_TAC [application] ]);
 
 val mainGeach' = store_thm ("mainGeach'",
-  ``!E A B C. extends L_Sequent E ==> gentzenSequent E (OneForm (Backslash B A))
-						       (Backslash (Backslash C B) (Backslash C A))``,
+  ``!E A B C. extends L_Sequent E
+	  ==> gentzenSequent E (OneForm (Backslash B A))
+			       (Backslash (Backslash C B) (Backslash C A))``,
     REPEAT STRIP_TAC
  >> NTAC 2 (MATCH_MP_TAC RightBackslash)
  >> MATCH_MP_TAC LextensionSimpl'
- >> CONJ_TAC THEN1 (POP_ASSUM ACCEPT_TAC)
+ >> CONJ_TAC
+ >- POP_ASSUM ACCEPT_TAC
  >> MATCH_MP_TAC CutRuleSimpl
  >> EXISTS_TAC ``(Dot B (Backslash B A))``
  >> CONJ_TAC
- >| [ MATCH_MP_TAC RightDot
-   >> CONJ_TAC
-   >| [ MATCH_MP_TAC LeftBackslashSimpl >> STRIP_TAC >> REWRITE_TAC [SeqAxiom],
+ >| [ MATCH_MP_TAC RightDot \\
+      CONJ_TAC >|
+      [ MATCH_MP_TAC LeftBackslashSimpl \\
+	STRIP_TAC \\
+	REWRITE_TAC [SeqAxiom],
 	REWRITE_TAC [SeqAxiom] ] ,
       REWRITE_TAC [application'] ]);
 
 val secondaryGeach = store_thm ("secondaryGeach",
-  ``!E A B C. extends L_Sequent E ==> gentzenSequent E (OneForm (Slash B C))
-						       (Backslash (Slash A B) (Slash A C))``,
+  ``!E A B C. extends L_Sequent E
+	  ==> gentzenSequent E (OneForm (Slash B C))
+			       (Backslash (Slash A B) (Slash A C))``,
     REPEAT STRIP_TAC
  >> MATCH_MP_TAC RightBackslash
  >> MATCH_MP_TAC RightSlash
  >> MATCH_MP_TAC LextensionSimpl
- >> CONJ_TAC THEN1 (POP_ASSUM ACCEPT_TAC)
+ >> CONJ_TAC >- (POP_ASSUM ACCEPT_TAC)
  >> MATCH_MP_TAC CutRuleSimpl
  >> EXISTS_TAC ``(Dot (Slash A B) B)``
  >> CONJ_TAC
- >| [ MATCH_MP_TAC RightDot
-   >> CONJ_TAC
-   >| [ REWRITE_TAC [SeqAxiom],
-	MATCH_MP_TAC LeftSlashSimpl >> STRIP_TAC >> REWRITE_TAC [SeqAxiom] ],
+ >| [ MATCH_MP_TAC RightDot \\
+      CONJ_TAC >|
+      [ REWRITE_TAC [SeqAxiom],
+	MATCH_MP_TAC LeftSlashSimpl \\
+	STRIP_TAC \\
+	REWRITE_TAC [SeqAxiom] ],
       REWRITE_TAC [application] ]);
 
 val secondaryGeach' = store_thm ("secondaryGeach'",
-``!E A B C. extends L_Sequent E ==> gentzenSequent E (OneForm (Backslash C B))
-						     (Slash (Backslash C A) (Backslash B A))``,
+``!E A B C. extends L_Sequent E
+	==> gentzenSequent E (OneForm (Backslash C B))
+			     (Slash (Backslash C A) (Backslash B A))``,
     REPEAT STRIP_TAC
  >> MATCH_MP_TAC RightSlash
  >> MATCH_MP_TAC RightBackslash
  >> MATCH_MP_TAC LextensionSimpl'
- >> CONJ_TAC THEN1 (POP_ASSUM ACCEPT_TAC)
+ >> CONJ_TAC
+ >- POP_ASSUM ACCEPT_TAC
  >> MATCH_MP_TAC CutRuleSimpl
  >> EXISTS_TAC ``(Dot B (Backslash B A))``
  >> CONJ_TAC
- >| [ MATCH_MP_TAC RightDot >> STRIP_TAC >|
-      [ MATCH_MP_TAC LeftBackslashSimpl >> STRIP_TAC >> REWRITE_TAC [SeqAxiom],
+ >| [ MATCH_MP_TAC RightDot \\
+      STRIP_TAC >|
+      [ MATCH_MP_TAC LeftBackslashSimpl \\
+	STRIP_TAC \\
+	REWRITE_TAC [SeqAxiom],
 	REWRITE_TAC [SeqAxiom] ] ,
       REWRITE_TAC [application'] ]);
 
 val composition = store_thm ("composition",
-  ``!E A B C. extends L_Sequent E ==> gentzenSequent E (OneForm (Dot (Slash A B) (Slash B C)))
-						       (Slash A C)``,
+  ``!E A B C. extends L_Sequent E
+	  ==> gentzenSequent E (OneForm (Dot (Slash A B) (Slash B C)))
+			       (Slash A C)``,
     REPEAT STRIP_TAC
  >> MATCH_MP_TAC CutRuleSimpl
  >> EXISTS_TAC ``(Dot (Slash (Slash A C) (Slash B C)) (Slash B C))``
  >> CONJ_TAC
- >| [ MATCH_MP_TAC monotonicity
-   >> CONJ_TAC >| [ RW_TAC bool_ss [mainGeach], REWRITE_TAC [SeqAxiom] ],
+ >| [ MATCH_MP_TAC monotonicity \\
+      CONJ_TAC >|
+      [ RW_TAC bool_ss [mainGeach], REWRITE_TAC [SeqAxiom] ],
       REWRITE_TAC [application] ]);
 
 val composition' = store_thm ("composition'",
-  ``!E A B C. extends L_Sequent E ==> gentzenSequent E (OneForm (Dot (Backslash C B) (Backslash B A)))
-						       (Backslash C A)``,
+  ``!E A B C. extends L_Sequent E
+	  ==> gentzenSequent E (OneForm (Dot (Backslash C B) (Backslash B A)))
+			       (Backslash C A)``,
     REPEAT STRIP_TAC
  >> MATCH_MP_TAC CutRuleSimpl
  >> EXISTS_TAC ``(Dot (Slash (Backslash C A) (Backslash B A)) (Backslash B A))``
  >> CONJ_TAC
- >| [ MATCH_MP_TAC monotonicity
-   >> CONJ_TAC >| [ RW_TAC bool_ss [secondaryGeach'], REWRITE_TAC [SeqAxiom] ],
+ >| [ MATCH_MP_TAC monotonicity \\
+      CONJ_TAC >|
+      [ RW_TAC bool_ss [secondaryGeach'], REWRITE_TAC [SeqAxiom] ],
       REWRITE_TAC [application] ]);
 
 val restructuring = store_thm ("restructuring",
-  ``!E A B C. extends L_Sequent E ==> gentzenSequent E (OneForm (Slash (Backslash A B) C))
-						       (Backslash A (Slash B C))``,
+  ``!E A B C. extends L_Sequent E
+	  ==> gentzenSequent E (OneForm (Slash (Backslash A B) C))
+			       (Backslash A (Slash B C))``,
     REPEAT STRIP_TAC
  >> MATCH_MP_TAC RightBackslash
  >> MATCH_MP_TAC RightSlash
  >> MATCH_MP_TAC LextensionSimpl
- >> CONJ_TAC THEN1 (POP_ASSUM ACCEPT_TAC)
+ >> CONJ_TAC
+ >- POP_ASSUM ACCEPT_TAC
  >> MATCH_MP_TAC CutRuleSimpl
  >> EXISTS_TAC ``(Dot A (Backslash A B))``
  >> CONJ_TAC
- >| [ MATCH_MP_TAC RightDot
-   >> CONJ_TAC THEN1 REWRITE_TAC [SeqAxiom]
-   >> MATCH_MP_TAC LeftSlashSimpl
-   >> REWRITE_TAC [SeqAxiom],
+ >| [ MATCH_MP_TAC RightDot \\
+      CONJ_TAC >| [ REWRITE_TAC [SeqAxiom],
+		    MATCH_MP_TAC LeftSlashSimpl \\
+		    REWRITE_TAC [SeqAxiom] ],
       REWRITE_TAC [application'] ]);
 
 val restructuring' = store_thm ("restructuring'",
-  ``!E A B C. extends L_Sequent E ==> gentzenSequent E (OneForm (Backslash A (Slash B C)))
-						       (Slash (Backslash A B) C)``,
+  ``!E A B C. extends L_Sequent E
+	  ==> gentzenSequent E (OneForm (Backslash A (Slash B C)))
+			       (Slash (Backslash A B) C)``,
     REPEAT STRIP_TAC
  >> MATCH_MP_TAC RightSlash
  >> MATCH_MP_TAC RightBackslash
  >> MATCH_MP_TAC LextensionSimpl'
- >> CONJ_TAC THEN1 POP_ASSUM ACCEPT_TAC
+ >> CONJ_TAC
+ >- POP_ASSUM ACCEPT_TAC
  >> MATCH_MP_TAC CutRuleSimpl
  >> EXISTS_TAC ``(Dot (Slash B C) C)``
  >> CONJ_TAC
- >| [ MATCH_MP_TAC RightDot
-   >> CONJ_TAC >| [ MATCH_MP_TAC LeftBackslashSimpl >> REWRITE_TAC [SeqAxiom],
+ >| [ MATCH_MP_TAC RightDot \\
+      CONJ_TAC >| [ MATCH_MP_TAC LeftBackslashSimpl \\
+		    REWRITE_TAC [SeqAxiom],
 		    REWRITE_TAC [SeqAxiom] ],
       REWRITE_TAC [application] ]);
 
 val currying = store_thm ("currying",
-  ``!E A B C. extends L_Sequent E ==> gentzenSequent E (OneForm (Slash A (Dot B C)))
-						       (Slash (Slash A C) B)``,
+  ``!E A B C. extends L_Sequent E
+	  ==> gentzenSequent E (OneForm (Slash A (Dot B C)))
+			       (Slash (Slash A C) B)``,
     REPEAT STRIP_TAC
  >> NTAC 2 (MATCH_MP_TAC RightSlashDot)
  >> MATCH_MP_TAC LextensionSimplDot
- >> CONJ_TAC THEN1 POP_ASSUM ACCEPT_TAC
+ >> CONJ_TAC
+ >- POP_ASSUM ACCEPT_TAC
  >> REWRITE_TAC [application]);
 
 val currying' = store_thm ("currying'",
-  ``!E A B C. extends L_Sequent E ==> gentzenSequent E (OneForm (Slash (Slash A C) B))
-						       (Slash A (Dot B C))``,
+  ``!E A B C. extends L_Sequent E
+	  ==> gentzenSequent E (OneForm (Slash (Slash A C) B))
+			       (Slash A (Dot B C))``,
     REPEAT STRIP_TAC
  >> MATCH_MP_TAC RightSlashDot
  >> MATCH_MP_TAC LextensionSimplDot'
- >> CONJ_TAC THEN1 POP_ASSUM ACCEPT_TAC
+ >> CONJ_TAC
+ >- POP_ASSUM ACCEPT_TAC
  >> MATCH_MP_TAC CutRuleSimpl
  >> EXISTS_TAC ``(Dot (Slash A C) C)``
  >> CONJ_TAC
@@ -1077,26 +1296,30 @@ val currying' = store_thm ("currying'",
       REWRITE_TAC [application] ]);
 
 val decurrying = store_thm ("decurrying",
-  ``!E A B C. extends L_Sequent E ==> gentzenSequent E (OneForm (Backslash (Dot A B) C))
-						       (Backslash B (Backslash A C))``,
+  ``!E A B C. extends L_Sequent E
+	  ==> gentzenSequent E (OneForm (Backslash (Dot A B) C))
+			       (Backslash B (Backslash A C))``,
     REPEAT STRIP_TAC
  >> NTAC 2 (MATCH_MP_TAC RightBackslashDot)
  >> MATCH_MP_TAC LextensionSimplDot'
- >> CONJ_TAC THEN1 POP_ASSUM ACCEPT_TAC
+ >> CONJ_TAC
+ >- POP_ASSUM ACCEPT_TAC
  >> REWRITE_TAC [application']);
 
 val decurrying' = store_thm ("decurrying'",
-  ``!E A B C. extends L_Sequent E ==> gentzenSequent E (OneForm (Backslash B (Backslash A C)))
-						       (Backslash (Dot A B) C)``,
+  ``!E A B C. extends L_Sequent E
+	  ==> gentzenSequent E (OneForm (Backslash B (Backslash A C)))
+			       (Backslash (Dot A B) C)``,
     REPEAT STRIP_TAC
  >> MATCH_MP_TAC RightBackslashDot
  >> MATCH_MP_TAC LextensionSimplDot
- >> CONJ_TAC THEN1 POP_ASSUM ACCEPT_TAC
+ >> CONJ_TAC
+ >- POP_ASSUM ACCEPT_TAC
  >> MATCH_MP_TAC CutRuleSimpl
  >> EXISTS_TAC ``(Dot A (Backslash A C))``
  >> CONJ_TAC
- >| [ MATCH_MP_TAC monotonicity
-   >> REWRITE_TAC [application', SeqAxiom],
+ >| [ MATCH_MP_TAC monotonicity \\
+      REWRITE_TAC [application', SeqAxiom],
       REWRITE_TAC [application'] ]);
 
 (* Theorem for systems that support commutativity: if its extension extends NLP_Sequent *)
@@ -1108,7 +1331,8 @@ val permutation = store_thm ("permutation",
     REPEAT STRIP_TAC
  >> MATCH_MP_TAC RightBackslashDot
  >> MATCH_MP_TAC NLPextensionSimplDot
- >> CONJ_TAC THEN1 ASM_REWRITE_TAC []
+ >> CONJ_TAC
+ >- ASM_REWRITE_TAC []
  >> MATCH_MP_TAC CutRuleSimpl
  >> EXISTS_TAC ``(Dot B (Backslash B C))``
  >> CONJ_TAC
@@ -1116,28 +1340,32 @@ val permutation = store_thm ("permutation",
       REWRITE_TAC [application'] ]);
 
 val exchange = store_thm ("exchange",
-  ``!E A B. extends NLP_Sequent E ==> gentzenSequent E (OneForm (Slash A B)) (Backslash B A)``,
+  ``!E A B. extends NLP_Sequent E
+	==> gentzenSequent E (OneForm (Slash A B)) (Backslash B A)``,
     REPEAT STRIP_TAC
  >> MATCH_MP_TAC RightBackslashDot
  >> MATCH_MP_TAC NLPextensionSimplDot
  >> RW_TAC bool_ss [application]);
 
 val exchange' = store_thm ("exchange'",
-  ``!E A B. extends NLP_Sequent E ==> gentzenSequent E (OneForm (Backslash B A)) (Slash A B)``,
+  ``!E A B. extends NLP_Sequent E
+	==> gentzenSequent E (OneForm (Backslash B A)) (Slash A B)``,
     REPEAT STRIP_TAC
  >> MATCH_MP_TAC RightSlashDot
  >> MATCH_MP_TAC NLPextensionSimplDot
  >> RW_TAC bool_ss [application']);
 
 val preposing = store_thm ("preposing",
-  ``!E A B. extends NLP_Sequent E ==> gentzenSequent E (OneForm A) (Slash B (Slash B A))``,
+  ``!E A B. extends NLP_Sequent E
+	==> gentzenSequent E (OneForm A) (Slash B (Slash B A))``,
     REPEAT STRIP_TAC
  >> MATCH_MP_TAC RightSlashDot
  >> MATCH_MP_TAC NLPextensionSimplDot
  >> RW_TAC bool_ss [application]);
 
 val postposing = store_thm ("postposing",
-  ``!E A B. extends NLP_Sequent E ==> gentzenSequent E (OneForm A) (Backslash (Backslash A B) B)``,
+  ``!E A B. extends NLP_Sequent E
+	==> gentzenSequent E (OneForm A) (Backslash (Backslash A B) B)``,
     REPEAT STRIP_TAC
  >> MATCH_MP_TAC RightBackslashDot
  >> MATCH_MP_TAC NLPextensionSimplDot
@@ -1150,35 +1378,882 @@ val mixedComposition = store_thm ("mixedComposition",
 	  ==> gentzenSequent E (OneForm (Dot (Slash A B) (Backslash C B))) (Backslash C A)``,
     REPEAT STRIP_TAC
  >> MATCH_MP_TAC NLPextensionSimplDot
- >> CONJ_TAC THEN1 (RW_TAC bool_ss [LPextendsNLP])
+ >> CONJ_TAC
+ >- RW_TAC bool_ss [LPextendsNLP]
  >> MATCH_MP_TAC RightBackslashDot
  >> MATCH_MP_TAC LextensionSimplDot'
- >> CONJ_TAC THEN1 (RW_TAC bool_ss [LPextendsL])
+ >> CONJ_TAC
+ >- RW_TAC bool_ss [LPextendsL]
  >> MATCH_MP_TAC CutRuleSimpl
  >> EXISTS_TAC ``(Dot B (Slash A B))``
  >> CONJ_TAC
- >| [ MATCH_MP_TAC monotonicity
-   >> RW_TAC bool_ss [application', SeqAxiom],
-      MATCH_MP_TAC NLPextensionSimplDot
-   >> RW_TAC bool_ss [application, LPextendsNLP] ]);
+ >| [ MATCH_MP_TAC monotonicity \\
+      RW_TAC bool_ss [application', SeqAxiom],
+      MATCH_MP_TAC NLPextensionSimplDot \\
+      RW_TAC bool_ss [application, LPextendsNLP] ]);
 
 val mixedComposition' = store_thm ("mixedComposition'",
   ``!E A B C. extends LP_Sequent E
 	 ==>  gentzenSequent E (OneForm (Dot (Slash B C) (Backslash B A))) (Slash A C)``,
     REPEAT STRIP_TAC
  >> MATCH_MP_TAC NLPextensionSimplDot
- >> CONJ_TAC THEN1 (RW_TAC bool_ss [LPextendsNLP])
+ >> CONJ_TAC
+ >- RW_TAC bool_ss [LPextendsNLP]
  >> MATCH_MP_TAC RightSlashDot
  >> MATCH_MP_TAC LextensionSimplDot
- >> CONJ_TAC THEN1 (RW_TAC bool_ss [LPextendsL])
+ >> CONJ_TAC
+ >- RW_TAC bool_ss [LPextendsL]
  >> MATCH_MP_TAC CutRuleSimpl
  >> EXISTS_TAC ``(Dot (Backslash B A) B)``
  >> CONJ_TAC
- >| [ MATCH_MP_TAC monotonicity
-   >> RW_TAC bool_ss [application, SeqAxiom],
-      MATCH_MP_TAC NLPextensionSimplDot
-   >> RW_TAC bool_ss [application', LPextendsNLP] ]);
+ >| [ MATCH_MP_TAC monotonicity \\
+      RW_TAC bool_ss [application, SeqAxiom],
+      MATCH_MP_TAC NLPextensionSimplDot \\
+      RW_TAC bool_ss [application', LPextendsNLP] ]);
+
+(******************************************************************************)
+(*                                                                            *)
+(*                          Module: ArrowGentzen                              *)
+(*                                                                            *)
+(******************************************************************************)
+
+val replace_arrow = store_thm ("replace_arrow",
+  ``!X Gamma Gamma' T1 T2.
+     replace Gamma Gamma' T1 T2 ==>
+     arrow X (deltaTranslation T2) (deltaTranslation T1) ==>
+     arrow X (deltaTranslation Gamma') (deltaTranslation Gamma)``,
+    GEN_TAC
+ >> HO_MATCH_MP_TAC replace_ind
+ >> REPEAT STRIP_TAC (* 2 sub-goals here *)
+ >| [ REWRITE_TAC [deltaTranslation_def] \\
+      RES_TAC \\
+      POP_ASSUM (ASSUME_TAC o (MATCH_MP Dot_mono_left)) \\
+      ASM_REWRITE_TAC [],
+      REWRITE_TAC [deltaTranslation_def] \\
+      RES_TAC \\
+      POP_ASSUM (ASSUME_TAC o (MATCH_MP Dot_mono_right)) \\
+      ASM_REWRITE_TAC [] ]);
+
+val replace_arrow' = store_thm ("replace_arrow'",
+  ``!C X Gamma Gamma' T1 T2.
+     replace Gamma Gamma' T1 T2 ==>
+     arrow X (deltaTranslation T2) (deltaTranslation T1) ==>
+     arrow X (deltaTranslation Gamma) C ==>
+     arrow X (deltaTranslation Gamma') C``,
+    REPEAT STRIP_TAC
+ >> IMP_RES_TAC replace_arrow
+ >> IMP_RES_TAC comp);
+
+(* from axiomatic presentation to sequent calculus *)
+val arrowToGentzenExt_def = Define `
+    arrowToGentzenExt (X :'a arrow_extension) (E :'a gentzen_extension) =
+	!A B. X A B ==> gentzenSequent E (OneForm A) B`;
+
+val NLToNL_Sequent = store_thm (
+   "NLToNL_Sequent", ``arrowToGentzenExt NL NL_Sequent``,
+    REWRITE_TAC [arrowToGentzenExt_def]
+ >> RW_TAC std_ss [NL_def, EMPTY_REL_DEF]);
+
+val NLPToNLP_Sequent = store_thm (
+   "NLPToNLP_Sequent", ``arrowToGentzenExt NLP NLP_Sequent``,
+    REWRITE_TAC [arrowToGentzenExt_def]
+ >> REWRITE_TAC [NLP_cases]
+ >> REPEAT STRIP_TAC
+ >> ASM_REWRITE_TAC []
+ >> ASSUME_TAC (ISPEC ``NLP_Sequent`` no_extend)
+ >> MATCH_MP_TAC NLPextensionSimplDot
+ >> ASM_REWRITE_TAC []
+ >> REWRITE_TAC [SeqAxiom]);
+
+val LToL_Sequent = store_thm (
+   "LToL_Sequent", ``arrowToGentzenExt L L_Sequent``,
+    REWRITE_TAC [arrowToGentzenExt_def]
+ >> REWRITE_TAC [L_cases]
+ >> ASSUME_TAC (ISPEC ``L_Sequent`` no_extend)
+ >> REPEAT STRIP_TAC (* 2 sub-goals here *)
+ >> ASM_REWRITE_TAC []
+ >| [ MATCH_MP_TAC LextensionSimplDot' >> ASM_REWRITE_TAC [] \\
+      REWRITE_TAC [SeqAxiom],
+      MATCH_MP_TAC LextensionSimplDot >> ASM_REWRITE_TAC [] \\
+      REWRITE_TAC [SeqAxiom] ]);
+
+val LPToLP_Sequent = store_thm (
+   "LPToLP_Sequent", ``arrowToGentzenExt LP LP_Sequent``,
+    REWRITE_TAC [arrowToGentzenExt_def, LP_def, RUNION]
+ >> REPEAT STRIP_TAC (* two sub-goals here *)
+ >| [ (* goal 1 (of 2) *)
+      MP_TAC NLP_Sequent_LP_Sequent \\
+      POP_ASSUM (MP_TAC o (MATCH_MP (REWRITE_RULE [arrowToGentzenExt_def] NLPToNLP_Sequent))) \\
+      REWRITE_TAC [mono_E],
+      (* goal 2 (of 2) *)
+      MP_TAC L_Sequent_LP_Sequent \\
+      POP_ASSUM (MP_TAC o (MATCH_MP (REWRITE_RULE [arrowToGentzenExt_def] LToL_Sequent))) \\
+      REWRITE_TAC [mono_E] ]);
+
+val arrowToGentzen = store_thm (
+   "arrowToGentzen",
+  ``!E X A B. arrow X A B ==> arrowToGentzenExt X E ==> gentzenSequent E (OneForm A) B``,
+    GEN_TAC
+ >> HO_MATCH_MP_TAC arrow_ind
+ >> REPEAT STRIP_TAC (* 7 goals here, first is easy *)
+ >- REWRITE_TAC [SeqAxiom] (* rest 6 goals *)
+ >| [ (* goal 1 (of 6) *)
+      MATCH_MP_TAC RightSlashDot >> RES_TAC,
+      (* goal 2 (of 6) *)
+      MATCH_MP_TAC DotRightSlash' >> RES_TAC,
+      (* goal 3 (of 6) *)
+      MATCH_MP_TAC RightBackslashDot >> RES_TAC,
+      (* goal 4 (of 6) *)
+      MATCH_MP_TAC DotRightBackslash' >> RES_TAC,
+      (* goal 5 (of 6) *)
+      MATCH_MP_TAC CutRuleSimpl \\
+      Q.EXISTS_TAC `A'` \\
+      RES_TAC \\
+      ASM_REWRITE_TAC [],
+      (* goal 6 (of 6) *)
+      POP_ASSUM (ASSUME_TAC o (REWRITE_RULE [arrowToGentzenExt_def])) \\
+      RES_TAC ]);
+
+(* particular cases for NLP, L; LP and NL systems *)
+val arrowToGentzenNL = store_thm (
+   "arrowToGentzenNL",
+  ``!A B. arrow NL A B ==> gentzenSequent NL_Sequent (OneForm A) B``,
+    REPEAT STRIP_TAC
+ >> irule arrowToGentzen
+ >> Q.EXISTS_TAC `NL`
+ >> ASM_REWRITE_TAC [NLToNL_Sequent]);
+
+val arrowToGentzenNLP = store_thm (
+   "arrowToGentzenNLP",
+  ``!A B. arrow NLP A B ==> gentzenSequent NLP_Sequent (OneForm A) B``,
+    REPEAT STRIP_TAC
+ >> irule arrowToGentzen
+ >> Q.EXISTS_TAC `NLP`
+ >> ASM_REWRITE_TAC [NLPToNLP_Sequent]);
+
+val arrowToGentzenL = store_thm (
+   "arrowToGentzenL",
+  ``!A B. arrow L A B ==> gentzenSequent L_Sequent (OneForm A) B``,
+    REPEAT STRIP_TAC
+ >> irule arrowToGentzen
+ >> Q.EXISTS_TAC `L`
+ >> ASM_REWRITE_TAC [LToL_Sequent]);
+
+val arrowToGentzenLP = store_thm (
+   "arrowToGentzenLP",
+  ``!A B. arrow LP A B ==> gentzenSequent LP_Sequent (OneForm A) B``,
+    REPEAT STRIP_TAC
+ >> irule arrowToGentzen
+ >> Q.EXISTS_TAC `LP`
+ >> ASM_REWRITE_TAC [LPToLP_Sequent]);
+
+(* from sequent calculus to axiomatic presentation.
+   Notice the strange thing here: the order of T1 and T2 are changed from E to X. *)
+val gentzenToArrowExt_def = Define
+   `gentzenToArrowExt (E :'a gentzen_extension) (X :'a arrow_extension) =
+	(!T1 T2. E T1 T2 ==> X (deltaTranslation T2) (deltaTranslation T1))`;
+
+(* Build arrow_extensions directly from gentzen_extensions *)
+val ToArrowExt_def = Define `
+    ToArrowExt (E :'a gentzen_extension) =
+	CURRY { (deltaTranslation y, deltaTranslation x) | (x,y) IN (UNCURRY E) }`;
+
+val ToArrowExt_thm = store_thm (
+   "ToArrowExt_thm",
+  ``!E T1 T2. E T1 T2 ==> (ToArrowExt E) (deltaTranslation T2) (deltaTranslation T1)``,
+    REPEAT STRIP_TAC
+ >> REWRITE_TAC [ToArrowExt_def, CURRY_DEF]
+ >> ONCE_REWRITE_TAC [GSYM SPECIFICATION]
+ >> ONCE_REWRITE_TAC [GSPECIFICATION]
+ >> Q.EXISTS_TAC `(T2, T1)`
+ >> `(T1, T2) IN (UNCURRY E)`
+	by PROVE_TAC [UNCURRY_DEF, SPECIFICATION]
+ >> FULL_SIMP_TAC std_ss []);
+
+val gentzenToArrowExt_thm = store_thm (
+   "gentzenToArrowExt_thm", ``!E. gentzenToArrowExt E (ToArrowExt E)``,
+    REWRITE_TAC [gentzenToArrowExt_def, ToArrowExt_thm]);
+
+val NL_SequentToNL = store_thm (
+   "NL_SequentToNL", ``gentzenToArrowExt NL_Sequent NL``,
+    REWRITE_TAC [gentzenToArrowExt_def]
+ >> RW_TAC std_ss [NL_Sequent_def, EMPTY_REL_DEF]);
+
+val NLP_SequentToNLP = store_thm (
+   "NLP_SequentToNLP", ``gentzenToArrowExt NLP_Sequent NLP``,
+    REWRITE_TAC [gentzenToArrowExt_def]
+ >> REWRITE_TAC [NLP_Sequent_cases]
+ >> REPEAT STRIP_TAC
+ >> ASM_REWRITE_TAC [deltaTranslation_def]
+ >> REWRITE_TAC [NLP_rules]);
+
+val L_SequentToL = store_thm (
+   "L_SequentToL", ``gentzenToArrowExt L_Sequent L``,
+    REWRITE_TAC [gentzenToArrowExt_def]
+ >> REWRITE_TAC [L_Sequent_cases]
+ >> REPEAT STRIP_TAC
+ >> ASM_REWRITE_TAC [deltaTranslation_def]
+ >| [ REWRITE_TAC [L_rule_lr],
+      REWRITE_TAC [L_rule_rl] ]);
+
+val LP_SequentToLP = store_thm (
+   "LP_SequentToLP", ``gentzenToArrowExt LP_Sequent LP``,
+    REWRITE_TAC [gentzenToArrowExt_def, LP_Sequent_def, RUNION]
+ >> REPEAT STRIP_TAC (* 2 sub-goals here *)
+ >| [ (* goal 1 (of 2) *)
+      POP_ASSUM (MP_TAC o (MATCH_MP (REWRITE_RULE [gentzenToArrowExt_def] NLP_SequentToNLP))) \\
+      MP_TAC NLPextendsLP \\
+      RW_TAC std_ss [RSUBSET],
+      (* goal 2 (of 2) *)
+      POP_ASSUM (MP_TAC o (MATCH_MP (REWRITE_RULE [gentzenToArrowExt_def] L_SequentToL))) \\
+      MP_TAC LextendsLP \\
+      RW_TAC std_ss [RSUBSET] ]);
+
+val gentzenToArrow' = store_thm (
+   "gentzenToArrow'",
+  ``!X E Gamma A. gentzenSequent E Gamma A ==> gentzenToArrowExt E X ==>
+		  arrow X (deltaTranslation Gamma) A``,
+    GEN_TAC
+ >> HO_MATCH_MP_TAC gentzenSequent_ind
+ >> REPEAT STRIP_TAC (* 9 sub-goals here *)
+ >| [ (* goal 1 *)
+      REWRITE_TAC [deltaTranslation_def, one],
+      (* goal 2 *)
+      RES_TAC >> POP_ASSUM MP_TAC \\
+      REWRITE_TAC [deltaTranslation_def, beta],
+      (* goal 3 *)
+      RES_TAC >> POP_ASSUM MP_TAC \\
+      REWRITE_TAC [deltaTranslation_def, gamma],
+      (* goal 4 *)
+      RES_TAC >> POP_ASSUM MP_TAC >> POP_ASSUM MP_TAC \\
+      RW_TAC std_ss [deltaTranslation_def, Dot_mono],
+      (* goal 5 *)
+      RES_TAC \\
+      SUFF_TAC ``arrow X (deltaTranslation (Comma (OneForm (Slash A A')) Gamma''))
+			 (deltaTranslation (OneForm A))`` >| (* 2 sub-goals here *)
+      [ (* goal 5.1 (of 2) *)
+	DISCH_TAC \\
+	`arrow X (deltaTranslation Gamma') (deltaTranslation Gamma)`
+		by PROVE_TAC [replace_arrow] \\
+	IMP_RES_TAC comp,
+	(* goal 5.2 (of 2) *)
+	REWRITE_TAC [deltaTranslation_def] \\
+	MATCH_MP_TAC beta' \\
+	MATCH_MP_TAC Slash_antimono_right \\
+	POP_ASSUM ACCEPT_TAC ],
+      (* goal 6 *)
+      RES_TAC \\
+      SUFF_TAC ``arrow X (deltaTranslation (Comma Gamma'' (OneForm (Backslash A' A))))
+			 (deltaTranslation (OneForm A))`` >| (* 2 sub-goals here *)
+      [ (* goal 6.1 (of 2) *)
+	DISCH_TAC \\
+	`arrow X (deltaTranslation Gamma') A''` by PROVE_TAC [replace_arrow'],
+	(* goal 6.2 (of 2) *)
+	REWRITE_TAC [deltaTranslation_def] \\
+	MATCH_MP_TAC gamma' \\
+	MATCH_MP_TAC Backslash_antimono_left \\
+	POP_ASSUM ACCEPT_TAC ],
+      (* goal 7 *)
+      RES_TAC \\
+      SUFF_TAC ``arrow X (deltaTranslation (OneForm (Dot A B)))
+			 (deltaTranslation (Comma (OneForm A) (OneForm B)))`` >|
+      (* 2 sub-goals here *)
+      [ (* goal 7.1 *)
+	DISCH_TAC \\
+	`arrow X (deltaTranslation Gamma') A'` by PROVE_TAC [replace_arrow'],
+	(* goal 7.2 *)
+	REWRITE_TAC [deltaTranslation_def, one] ],
+     (* goal 8 *)
+     RES_TAC \\
+     `arrow X (deltaTranslation Gamma) (deltaTranslation (OneForm A))`
+	by ASM_REWRITE_TAC [deltaTranslation_def] \\
+     `arrow X (deltaTranslation Gamma'') A'` by PROVE_TAC [replace_arrow'],
+     (* goal 9 *)
+     FULL_SIMP_TAC std_ss [gentzenToArrowExt_def] \\
+     RES_TAC \\
+     `arrow X (deltaTranslation Delta') (deltaTranslation Delta)`
+	by PROVE_TAC [arrow_plus] \\
+     `arrow X (deltaTranslation Gamma') A` by PROVE_TAC [replace_arrow'] ]);
+
+val gentzenToArrow = store_thm (
+   "gentzenToArrow",
+  ``!E X Gamma A. gentzenToArrowExt E X /\ gentzenSequent E Gamma A
+	      ==> arrow X (deltaTranslation Gamma) A``,
+    REPEAT STRIP_TAC
+ >> PAT_X_ASSUM ``gentzenToArrowExt E X`` MP_TAC
+ >> POP_ASSUM MP_TAC
+ >> REWRITE_TAC [gentzenToArrow']);
+
+val gentzenToArrow_E = store_thm (
+   "gentzenToArrow_E",
+  ``!E Gamma A. gentzenSequent E Gamma A ==> arrow (ToArrowExt E) (deltaTranslation Gamma) A``,
+    REPEAT STRIP_TAC
+ >> ASSUME_TAC (Q.SPEC `E` gentzenToArrowExt_thm)
+ >> NTAC 2 (POP_ASSUM MP_TAC)
+ >> REWRITE_TAC [gentzenToArrow']);
+
+val NLGentzenToArrow = store_thm (
+   "NLGentzenToArrow",
+  ``!Gamma A. gentzenSequent NL_Sequent Gamma A ==> arrow NL (deltaTranslation Gamma) A``,
+    REPEAT STRIP_TAC
+ >> MP_TAC NL_SequentToNL
+ >> POP_ASSUM MP_TAC
+ >> REWRITE_TAC [gentzenToArrow']);
+
+val NLPGentzenToArrow = store_thm (
+   "NLPGentzenToArrow",
+  ``!Gamma A. gentzenSequent NLP_Sequent Gamma A ==> arrow NLP (deltaTranslation Gamma) A``,
+    REPEAT STRIP_TAC
+ >> MP_TAC NLP_SequentToNLP
+ >> POP_ASSUM MP_TAC
+ >> REWRITE_TAC [gentzenToArrow']);
+
+val LGentzenToArrow = store_thm (
+   "LGentzenToArrow",
+  ``!Gamma A. gentzenSequent L_Sequent Gamma A ==> arrow L (deltaTranslation Gamma) A``,
+    REPEAT STRIP_TAC
+ >> MP_TAC L_SequentToL
+ >> POP_ASSUM MP_TAC
+ >> REWRITE_TAC [gentzenToArrow']);
+
+val LPGentzenToArrow = store_thm (
+   "LPGentzenToArrow",
+  ``!Gamma A. gentzenSequent LP_Sequent Gamma A ==> arrow LP (deltaTranslation Gamma) A``,
+    REPEAT STRIP_TAC
+ >> MP_TAC LP_SequentToLP
+ >> POP_ASSUM MP_TAC
+ >> REWRITE_TAC [gentzenToArrow']);
+
+(******************************************************************************)
+(*                                                                            *)
+(*          Module: Gentzen's Sequent Calculus and Natural Deduction          *)
+(*                                                                            *)
+(******************************************************************************)
+
+val replaceGentzen = store_thm ("replaceGentzen",
+  ``!E Gamma Gamma' Delta Delta'.
+     replace Gamma Gamma' Delta Delta' ==>
+     gentzenSequent E Delta' (deltaTranslation Delta) ==>
+     gentzenSequent E Gamma' (deltaTranslation Gamma)``,
+    X_GEN_TAC ``E :'a gentzen_extension``
+ >> Induct_on `replace`
+ >> REPEAT STRIP_TAC
+ >> `gentzenSequent E Delta (deltaTranslation Delta)` by PROVE_TAC [SeqAxiomGeneralized]
+ >> `gentzenSequent E Gamma' (deltaTranslation Gamma)` by PROVE_TAC []
+ >> PROVE_TAC [RightDot, deltaTranslation_def]);
+
+val replaceGentzen' = store_thm (
+   "replaceGentzen'",
+  ``!Gamma Gamma' Delta Delta' C E.
+     replace Gamma Gamma' Delta Delta' /\
+     gentzenSequent E Delta' (deltaTranslation Delta) /\
+     gentzenSequent E Gamma C ==>
+     gentzenSequent E Gamma' C``,
+    REPEAT STRIP_TAC
+ >> MATCH_MP_TAC CutRuleSimpl
+ >> EXISTS_TAC ``(deltaTranslation Gamma)``
+ >> CONJ_TAC (* 2 sub-goals here *)
+ >| [ (* goal 1 (of 2) *)
+      IMP_RES_TAC replaceGentzen,
+      (* goal 2 (of 2) *)
+      MATCH_MP_TAC SeqTermToForm \\
+      ASM_REWRITE_TAC [] ]);
+
+val replaceNatDed = store_thm ("replaceNatDed",
+  ``!E Gamma Gamma' Delta Delta'.
+    replace Gamma Gamma' Delta Delta' ==>
+    natDed E Delta' (deltaTranslation Delta) ==>
+    natDed E Gamma' (deltaTranslation Gamma)``,
+    GEN_TAC
+ >> HO_MATCH_MP_TAC replace_ind
+ >> CONJ_TAC
+ >- RW_TAC bool_ss []
+ >> REWRITE_TAC [deltaTranslation_def]
+ >> CONJ_TAC
+ >> REPEAT STRIP_TAC
+ >> MATCH_MP_TAC DotIntro
+ >> RW_TAC bool_ss [NatAxiomGeneralized]);
+
+(* easier for MATCH_MP_TAC *)
+val replaceNatDed' = store_thm (
+   "replaceNatDed'",
+  ``!E Gamma Gamma' Delta Delta'.
+     replace Gamma Gamma' Delta Delta' /\
+     natDed E Delta' (deltaTranslation Delta) ==>
+     natDed E Gamma' (deltaTranslation Gamma)``,
+    REPEAT STRIP_TAC
+ >> NTAC 2 (POP_ASSUM MP_TAC)
+ >> REWRITE_TAC [replaceNatDed]);
+
+(* E T1[A] T2[A] ==> ?T1[Delta]. X T1[Delta] T2[Delta] *)
+val condCutExt_def = Define `
+    condCutExt (E :'a gentzen_extension) =
+	!Gamma T1 T2 A Delta.
+	 E T1 T2 ==> replace T2 Gamma (OneForm A) Delta
+	         ==> ?Gamma'. E Gamma' Gamma /\ replace T1 Gamma' (OneForm A) Delta`;
+
+val conditionOKNL = store_thm ("conditionOKNL", ``condCutExt NL_Sequent``,
+    REWRITE_TAC [condCutExt_def]
+ >> REPEAT GEN_TAC
+ >> GEN_REWRITE_TAC (RATOR_CONV o ONCE_DEPTH_CONV) empty_rewrites [NL_Sequent_def]
+ >> RW_TAC std_ss [EMPTY_REL_DEF]);
+
+val conditionOKNLP = store_thm ("conditionOKNLP", ``condCutExt NLP_Sequent``,
+    REWRITE_TAC [condCutExt_def]
+ >> REPEAT GEN_TAC
+ >> GEN_REWRITE_TAC (RATOR_CONV o ONCE_DEPTH_CONV) empty_rewrites [NLP_Sequent_cases]
+ >> REPEAT STRIP_TAC
+ >> `replace (Comma B A') Gamma (OneForm A) Delta` by PROVE_TAC []
+ >> ASM_REWRITE_TAC []
+ >> POP_ASSUM (MP_TAC o (MATCH_MP replace_inv2))
+ >> REPEAT STRIP_TAC (* 2 sub-goals here *)
+ >| [ (* goal 1 (of 2) *)
+      ASM_REWRITE_TAC [] \\
+      EXISTS_TAC ``(Comma A' G)`` \\
+      CONJ_TAC >| (* 2 sub-goals here *)
+      [ REWRITE_TAC [NLP_Sequent_rules],
+        MATCH_MP_TAC replaceRight >> ASM_REWRITE_TAC [] ],
+      ASM_REWRITE_TAC [] \\
+      EXISTS_TAC ``(Comma G B)`` \\
+      CONJ_TAC >| (* 2 sub-goals here *)
+      [ REWRITE_TAC [NLP_Sequent_rules],
+        MATCH_MP_TAC replaceLeft >> ASM_REWRITE_TAC [] ] ]);
+
+val conditionOKL = store_thm ("conditionOKL", ``condCutExt L_Sequent``,
+    REWRITE_TAC [condCutExt_def]
+ >> REPEAT GEN_TAC
+ >> GEN_REWRITE_TAC (RATOR_CONV o ONCE_DEPTH_CONV) empty_rewrites [L_Sequent_cases]
+ >> REPEAT STRIP_TAC (* 2 sub-goals here *)
+ >| [ (* goal 1 *)
+      ASM_REWRITE_TAC []						\\
+      `replace (Comma (Comma A' B) C) Gamma (OneForm A) Delta`
+	by PROVE_TAC []							\\
+      POP_ASSUM (MP_TAC o (MATCH_MP replace_inv2))			\\
+      REPEAT STRIP_TAC >| (* 2 sub sub-goals here *)
+      [ (* goal 1.1 (of 2) *)
+	POP_ASSUM (MP_TAC o (MATCH_MP replace_inv2))			\\
+	REPEAT STRIP_TAC >| (* 2 sub-goals here *)
+	[ (* goal 1.1.1 (of 2) *)
+	  ASM_REWRITE_TAC []						\\
+	  EXISTS_TAC ``(Comma G' (Comma B C))``				\\
+	  CONJ_TAC >- REWRITE_TAC [L_Sequent_rules]			\\
+	  MATCH_MP_TAC replaceLeft					\\
+	  ASM_REWRITE_TAC [],
+	  (* goal 1.1.2 (of 2) *)
+	  ASM_REWRITE_TAC []						\\
+	  EXISTS_TAC ``(Comma A' (Comma G' C))``			\\
+	  CONJ_TAC >- REWRITE_TAC [L_Sequent_rules]			\\
+	  MATCH_MP_TAC replaceRight					\\
+	  MATCH_MP_TAC replaceLeft					\\
+	  ASM_REWRITE_TAC [] ],
+	(* goal 1.2 (of 2) *)
+	ASM_REWRITE_TAC []						\\
+	EXISTS_TAC ``(Comma A' (Comma B G))``				\\
+	CONJ_TAC >- REWRITE_TAC [L_Sequent_rules]			\\
+	NTAC 2 (MATCH_MP_TAC replaceRight)				\\
+        ASM_REWRITE_TAC [] ],
+      (* goal 2 (of 2) *)
+      ASM_REWRITE_TAC []						\\
+      `replace (Comma A' (Comma B C)) Gamma (OneForm A) Delta`
+	by PROVE_TAC []							\\
+      POP_ASSUM (MP_TAC o (MATCH_MP replace_inv2))			\\
+      REPEAT STRIP_TAC >| (* 2 sub-goals here *)
+      [ (* goal 2.1 (of 2) *)
+	ASM_REWRITE_TAC []						\\
+	EXISTS_TAC ``(Comma (Comma G B) C)``				\\
+	CONJ_TAC >- REWRITE_TAC [L_Sequent_rules]			\\
+	NTAC 2 (MATCH_MP_TAC replaceLeft)				\\
+	ASM_REWRITE_TAC [],
+	(* goal 2.2 (of 2) *)
+	POP_ASSUM (MP_TAC o (MATCH_MP replace_inv2))			\\
+	REPEAT STRIP_TAC >| (* 2 sub-goals here *)
+	[ (* goal 2.2.1 (of 2) *)
+	  ASM_REWRITE_TAC []						\\
+	  EXISTS_TAC ``(Comma (Comma A' G') C)``			\\
+	  CONJ_TAC >- REWRITE_TAC [L_Sequent_rules]			\\
+	  MATCH_MP_TAC replaceLeft					\\
+	  MATCH_MP_TAC replaceRight					\\
+	  ASM_REWRITE_TAC [],
+	  (* goal 2.2.2 (of 2) *)
+	  ASM_REWRITE_TAC []						\\
+	  EXISTS_TAC ``(Comma (Comma A' B) G')``			\\
+	  CONJ_TAC >- REWRITE_TAC [L_Sequent_rules]			\\
+	  MATCH_MP_TAC replaceRight					\\
+	  ASM_REWRITE_TAC [] ] ] ]);
+
+val condAddExt = store_thm (
+   "condAddExt",
+  ``!E E'. condCutExt E /\ condCutExt E' ==> condCutExt (add_extension E E')``,
+    REPEAT GEN_TAC
+ >> REWRITE_TAC [condCutExt_def, RUNION]
+ >> REPEAT STRIP_TAC (* 2 sub-goals here *)
+ >| [ (* goal 1 (of 2) *)
+      RES_TAC >> Q.EXISTS_TAC `Gamma'` \\
+      ASM_REWRITE_TAC [],
+      (* goal 2 (of 2) *)
+      RES_TAC >> Q.EXISTS_TAC `Gamma'` \\
+      ASM_REWRITE_TAC [] ]);
+
+val CutNatDed = store_thm (
+   "CutNatDed",
+  ``!Delta A E Gamma C. natDed E Gamma C ==> condCutExt E ==> natDed E Delta A ==>
+	!Gamma'. replace Gamma Gamma' (OneForm A) Delta ==> natDed E Gamma' C``,
+    NTAC 2 GEN_TAC
+ >> Induct_on `natDed`
+ >> REPEAT STRIP_TAC (* 8 sub-goals here *)
+ >| [ (* goal 1 (of 8) *)
+      POP_ASSUM (MP_TAC o (MATCH_MP replace_inv1))			\\
+      RW_TAC std_ss []							\\
+      ASM_REWRITE_TAC [],
+      (* goal 2 (of 8) *)
+      MATCH_MP_TAC SlashIntro						\\
+      IMP_RES_TAC replaceLeft						\\
+      POP_ASSUM (ASSUME_TAC o (SPEC ``(OneForm B)``)) >> RES_TAC,
+      (* goal 3 (of 8) *)
+      MATCH_MP_TAC BackslashIntro					\\
+      IMP_RES_TAC replaceRight						\\
+      POP_ASSUM (ASSUME_TAC o (SPEC ``(OneForm B)``)) >> RES_TAC,
+      (* goal 4 (of 8) *)
+      POP_ASSUM (MP_TAC o (MATCH_MP replace_inv2))			\\
+      REPEAT STRIP_TAC >| (* 2 sub-goals here *)
+      [ (* goal 4.1 (of 2) *)
+        ASM_REWRITE_TAC []						\\
+        MATCH_MP_TAC DotIntro						\\
+        CONJ_TAC >- RES_TAC						\\
+        ASM_REWRITE_TAC [],
+        (* goal 4.2 (of 2) *)
+        ASM_REWRITE_TAC []						\\
+        MATCH_MP_TAC DotIntro						\\
+        CONJ_TAC >- ASM_REWRITE_TAC []					\\
+        RES_TAC ],
+      (* goal 5 (of 8) *)
+      POP_ASSUM (MP_TAC o (MATCH_MP replace_inv2))			\\
+      REPEAT STRIP_TAC (* 2 sub-goals here, same tacticals *)		\\
+      ASM_REWRITE_TAC []						\\
+      MATCH_MP_TAC SlashElim						\\
+      Q.EXISTS_TAC `C'`	(* NOTE: expk needs `C''` here! *)		\\
+      ASM_REWRITE_TAC [] >> RES_TAC,
+      (* goal 6 (of 8) *)
+      POP_ASSUM (MP_TAC o (MATCH_MP replace_inv2))			\\
+      REPEAT STRIP_TAC (* 2 sub-goals here, same tacticals *)		\\
+      ASM_REWRITE_TAC []						\\
+      MATCH_MP_TAC BackslashElim					\\
+      Q.EXISTS_TAC `C'`	(* NOTE: expk needs `C''` here! *)		\\
+      ASM_REWRITE_TAC [] >> RES_TAC,
+      (* goal 7 (of 8) *)
+      PAT_X_ASSUM ``replace Gamma Gamma' (Comma (OneForm A') (OneForm B)) Gamma''``
+	(ASSUME_TAC o (MATCH_MP doubleReplace))				\\
+      POP_ASSUM (ASSUME_TAC o (Q.SPECL [`Gamma'''`, `A`, `Delta`]))	\\
+      RES_TAC (* 2 sub-goals here, same tactical *)			\\
+      IMP_RES_TAC DotElim,
+      (* goal 8 (of 8) *)
+      PAT_X_ASSUM ``condCutExt E ==> P``
+	(ASSUME_TAC o
+	  (fn thm => (MATCH_MP thm (ASSUME ``condCutExt E``))))		\\
+      PAT_X_ASSUM ``natDed E Delta A ==> P``
+	(ASSUME_TAC o
+	  (fn thm => (MATCH_MP thm (ASSUME ``natDed E Delta A``))))	\\
+      PAT_X_ASSUM ``condCutExt E``
+	(ASSUME_TAC o (REWRITE_RULE [condCutExt_def]))			\\
+      PAT_X_ASSUM ``replace Gamma Gamma' Delta' Delta''``
+	(ASSUME_TAC o (MATCH_MP doubleReplace))				\\
+      POP_ASSUM (ASSUME_TAC o (Q.SPECL [`Gamma''`, `A`, `Delta`]))	\\
+      POP_ASSUM (MP_TAC o
+	(fn thm => (MATCH_MP
+		     thm (ASSUME ``replace Gamma' Gamma'' (OneForm A) Delta``)))) \\
+      REPEAT STRIP_TAC >| (* 2 sub-goals here *)
+      [ (* goal 8.1 (of 2) *)
+	MATCH_MP_TAC NatExt						\\
+	Q.EXISTS_TAC `G`						\\
+	Q.EXISTS_TAC `Delta'`						\\
+	Q.EXISTS_TAC `Delta''`						\\
+	CONJ_TAC >- ASM_REWRITE_TAC []					\\
+	CONJ_TAC >- ASM_REWRITE_TAC []					\\
+	PAT_X_ASSUM ``!Gamma'. replace Gamma Gamma' (OneForm A) Delta ==> P``
+	  (ASSUME_TAC o (Q.SPEC `G`))					\\
+	RES_TAC,
+        (* goal 8.2 (of 2) *)
+        PAT_X_ASSUM ``!Gamma T1 T2 A Delta. E T1 T2 ==> P``
+	  (ASSUME_TAC o
+	    (Q.SPECL [`G`, `Delta'`, `Delta''`, `A`, `Delta`]))		\\
+        POP_ASSUM (ASSUME_TAC o
+	  (fn thm => (MP thm (ASSUME ``(E :'a gentzen_extension) Delta' Delta''``)))) \\
+        POP_ASSUM (ASSUME_TAC o
+	  (fn thm => (MP thm (ASSUME ``replace Delta'' G (OneForm A) Delta``)))) \\
+        POP_ASSUM MP_TAC >> STRIP_TAC					\\
+        PAT_X_ASSUM ``replace Gamma Gamma'' Delta' G``
+	  (ASSUME_TAC o (MATCH_MP replaceSameP))			\\
+        POP_ASSUM (ASSUME_TAC o (Q.SPEC `Gamma'''`))			\\
+        POP_ASSUM MP_TAC >> STRIP_TAC					\\
+        MATCH_MP_TAC NatExt						\\
+        Q.EXISTS_TAC `G'` (* NOTE: expk needs `G''` here! *)		\\
+        Q.EXISTS_TAC `Gamma'''`						\\
+        Q.EXISTS_TAC `G`						\\
+        CONJ_TAC >- ASM_REWRITE_TAC []					\\
+        CONJ_TAC >- ASM_REWRITE_TAC []					\\
+        PAT_X_ASSUM ``!Gamma'. P`` MATCH_MP_TAC				\\
+        MATCH_MP_TAC replaceTrans'					\\
+        Q.EXISTS_TAC `Delta'`						\\
+        Q.EXISTS_TAC `Gamma'''`						\\
+        CONJ_TAC >- ASM_REWRITE_TAC []					\\
+        ASM_REWRITE_TAC [] ] ] );
+
+val natDedComposition = store_thm (
+   "natDedComposition",
+  ``!E Gamma F1 F2. condCutExt E /\ natDed E Gamma F1 /\ natDed E (OneForm F1) F2
+		==> natDed E Gamma F2``,
+    REPEAT STRIP_TAC
+ >> irule CutNatDed >- ASM_REWRITE_TAC []
+ >> Q.EXISTS_TAC `F1`
+ >> Q.EXISTS_TAC `Gamma`
+ >> Q.EXISTS_TAC `(OneForm F1)`
+ >> RW_TAC std_ss [replaceRoot]);
+
+(* The easy direction, doesn't depend on new theorems in this section *)
+val natDedToGentzen = store_thm (
+   "natDedToGentzen",
+  ``!E Gamma C. natDed E Gamma C ==> gentzenSequent E Gamma C``,
+    HO_MATCH_MP_TAC natDed_ind (* or: Induct_on `natDed` *)
+ >> REPEAT STRIP_TAC (* 8 sub-goals here *)
+ >| [ (* goal 1 (of 8) *)
+      REWRITE_TAC [SeqAxiom],
+      (* goal 2 (of 8) *)
+      MATCH_MP_TAC RightSlash						\\
+      ASM_REWRITE_TAC [],
+      (* goal 3 (of 8) *)
+      MATCH_MP_TAC RightBackslash					\\
+      ASM_REWRITE_TAC [],
+      (* goal 4 (of 8) *)
+      MATCH_MP_TAC RightDot						\\
+      ASM_REWRITE_TAC [],
+      (* goal 5 (of 8) *)
+      MATCH_MP_TAC CutRule						\\
+      Q.EXISTS_TAC `Gamma` (* for Delta' *)				\\
+      EXISTS_TAC ``(Comma (OneForm (Slash A B)) Delta)``		\\
+      EXISTS_TAC ``(Slash A B)``					\\
+      CONJ_TAC >| (* 2 sub-goals here *)
+      [ (* goal 5.1 (of 2) *)
+        MATCH_MP_TAC replaceLeft					\\
+        REWRITE_TAC [replaceRoot],
+        (* goal 5.2 (of 2) *)
+        CONJ_TAC >- ASM_REWRITE_TAC []					\\
+        MATCH_MP_TAC LeftSlashSimpl					\\
+        CONJ_TAC >- ASM_REWRITE_TAC []					\\
+        REWRITE_TAC [SeqAxiom] ],
+      (* goal 6 (of 8) *)
+      MATCH_MP_TAC CutRule						\\
+      Q.EXISTS_TAC `Delta`						\\
+      EXISTS_TAC ``(Comma Gamma (OneForm (Backslash B A)))``		\\
+      EXISTS_TAC ``(Backslash B A)``					\\
+      CONJ_TAC >| (* 2 sub-goals here *)
+      [ (* goal 6.1 (of 2) *)
+        MATCH_MP_TAC replaceRight					\\
+        REWRITE_TAC [replaceRoot],
+        (* goal 6.2 (of 2) *)
+        CONJ_TAC >- ASM_REWRITE_TAC []					\\
+        MATCH_MP_TAC LeftBackslashSimpl					\\
+        CONJ_TAC >- ASM_REWRITE_TAC []					\\
+        REWRITE_TAC [SeqAxiom] ],
+      (* goal 7 (of 8) *)
+      MATCH_MP_TAC replaceGentzen'					\\
+      Q.EXISTS_TAC `Gamma`						\\
+      EXISTS_TAC ``(Comma (OneForm A) (OneForm B))``			\\
+      Q.EXISTS_TAC `Delta`						\\
+      CONJ_TAC >- ASM_REWRITE_TAC []					\\
+      REWRITE_TAC [deltaTranslation_def]				\\
+      CONJ_TAC >- ASM_REWRITE_TAC []					\\
+      ASM_REWRITE_TAC [],
+      (* goal 8 (of 8) *)
+      MP_TAC (SPEC_ALL SeqExt) >> REPEAT STRIP_TAC			\\
+      RES_TAC ]);
+
+(* The hard direction, heavily depends on theorems proved recently *)
+val gentzenToNatDed = store_thm (
+   "gentzenToNatDed",
+  ``!E Gamma C. gentzenSequent E Gamma C ==> condCutExt E ==> natDed E Gamma C``,
+    HO_MATCH_MP_TAC gentzenSequent_ind (* or: Induct_on `gentzenSequent` *)
+ >> REPEAT STRIP_TAC (* 9 sub-goals here *)
+ >| [ (* goal 1 (of 9) *)
+      REWRITE_TAC [NatAxiom],
+      (* goal 2 (of 9) *)
+      RES_TAC								\\
+      MATCH_MP_TAC SlashIntro >> ASM_REWRITE_TAC [],
+      (* goal 3 (of 9) *)
+      RES_TAC								\\
+      MATCH_MP_TAC BackslashIntro >> ASM_REWRITE_TAC [],
+      (* goal 4 (of 9) *)
+      RES_TAC								\\
+      MATCH_MP_TAC DotIntro >> ASM_REWRITE_TAC [],
+      (* goal 5 (of 9) *)
+      MATCH_MP_TAC natDedComposition					\\
+      EXISTS_TAC ``(deltaTranslation Gamma)``				\\
+      CONJ_TAC >- ASM_REWRITE_TAC []					\\
+      CONJ_TAC >| (* 2 sub-goals here *)
+      [ (* goal 5.1 (of 2) *)
+        MATCH_MP_TAC replaceNatDed'					\\
+        EXISTS_TAC ``(OneForm A)``					\\
+        (* NOTE: expk needs `...(Slash A C')...` here! *)
+        EXISTS_TAC ``(Comma (OneForm (Slash A C)) Gamma'')``		\\
+        CONJ_TAC >- ASM_REWRITE_TAC []					\\
+        REWRITE_TAC [deltaTranslation_def]				\\
+        MATCH_MP_TAC SlashElim						\\
+        Q.EXISTS_TAC `C` (* NOTE: expk needs `C'` here! *)		\\
+        CONJ_TAC >- REWRITE_TAC [NatAxiom] >> RES_TAC,
+        (* goal 5.2 (of 2) *)
+        MATCH_MP_TAC NatTermToForm >> RES_TAC ],
+      (* goal 6 (of 9) *)
+      MATCH_MP_TAC natDedComposition					\\
+      EXISTS_TAC ``(deltaTranslation Gamma)``				\\
+      CONJ_TAC >- ASM_REWRITE_TAC []					\\
+      CONJ_TAC >| (* 2 sub-goals here *)
+      [ (* goal 6.1 (of 2) *)
+        MATCH_MP_TAC replaceNatDed'					\\
+        EXISTS_TAC ``(OneForm A)``					\\
+        (* NOTE: expk needs `...(Backslash C' A)...` here! *)
+        EXISTS_TAC ``(Comma Gamma'' (OneForm (Backslash C A)))``	\\
+        CONJ_TAC >- ASM_REWRITE_TAC []					\\
+        REWRITE_TAC [deltaTranslation_def]				\\
+        MATCH_MP_TAC BackslashElim					\\
+        Q.EXISTS_TAC `C` (* NOTE: expk needs `C'` here! *)		\\
+        CONJ_TAC >- RES_TAC						\\
+        REWRITE_TAC [NatAxiom],
+        (* goal 6.2 (of 2) *)
+        MATCH_MP_TAC NatTermToForm >> RES_TAC ],
+      (* goal 7 (of 9) *)
+      MATCH_MP_TAC natDedComposition					\\
+      EXISTS_TAC ``(deltaTranslation Gamma)``				\\
+      CONJ_TAC >- ASM_REWRITE_TAC []					\\
+      CONJ_TAC >| (* 2 sub-goals here *)
+      [ (* goal 7.1 (of 2) *)
+        MATCH_MP_TAC replaceNatDed'					\\
+        EXISTS_TAC ``(Comma (OneForm A) (OneForm B))``			\\
+        EXISTS_TAC ``(OneForm (Dot A B))``				\\
+        CONJ_TAC >- ASM_REWRITE_TAC []					\\
+        REWRITE_TAC [deltaTranslation_def]				\\
+        REWRITE_TAC [NatAxiom],
+        (* goal 7.2 (of 2) *)
+        MATCH_MP_TAC NatTermToForm >> RES_TAC ],
+      (* goal 8 (of 9) *)
+      MATCH_MP_TAC natDedComposition					\\
+      EXISTS_TAC ``(deltaTranslation Gamma')``				\\
+      CONJ_TAC >- ASM_REWRITE_TAC []					\\
+      CONJ_TAC >| (* 2 sub-goals here *)
+      [ (* goal 8.1 (of 2) *)
+        MATCH_MP_TAC replaceNatDed'					\\
+        EXISTS_TAC ``(OneForm C)`` (* NOTE: expk needs `C'` here! *)	\\
+        Q.EXISTS_TAC `Gamma`						\\
+        CONJ_TAC >- ASM_REWRITE_TAC []					\\
+        REWRITE_TAC [deltaTranslation_def] >> RES_TAC,
+        (* goal 8.2 (of 2) *)
+        MATCH_MP_TAC NatTermToForm >> RES_TAC ],
+      (* goal 9 (of 9) *)
+      MATCH_MP_TAC NatExt						\\
+      Q.EXISTS_TAC `Gamma`						\\
+      Q.EXISTS_TAC `Delta`						\\
+      Q.EXISTS_TAC `Delta'`						\\
+      CONJ_TAC >- ASM_REWRITE_TAC []					\\
+      CONJ_TAC >- ASM_REWRITE_TAC []					\\
+      RES_TAC ]);
+
+val gentzenEqNatDed = store_thm (
+   "gentzenEqNatDed",
+  ``!E Gamma C. condCutExt E ==> (gentzenSequent E Gamma C = natDed E Gamma C)``,
+    REPEAT STRIP_TAC
+ >> EQ_TAC (* 2 sub-goals here *)
+ >| [ (* goal 1 (of 2) *)
+      DISCH_TAC \\
+      irule gentzenToNatDed \\ (* 2 sub-goals sharing the same tactical *)
+      ASM_REWRITE_TAC [],
+      (* goal 2 (of 2) *)
+      REWRITE_TAC [natDedToGentzen] ]);
+
+val NLgentzenEqNatDed = store_thm (
+   "NLgentzenEqNatDed",
+  ``!Gamma C. gentzenSequent NL_Sequent Gamma C = natDed NL_Sequent Gamma C``,
+    REPEAT STRIP_TAC
+ >> MP_TAC conditionOKNL
+ >> REWRITE_TAC [gentzenEqNatDed]);
+
+val LgentzenEqNatDed = store_thm (
+   "LgentzenEqNatDed",
+  ``!Gamma C. gentzenSequent L_Sequent Gamma C = natDed L_Sequent Gamma C``,
+    REPEAT STRIP_TAC
+ >> MP_TAC conditionOKL
+ >> REWRITE_TAC [gentzenEqNatDed]);
+
+val NLPgentzenEqNatDed = store_thm (
+   "NLPgentzenEqNatDed",
+ ``!Gamma C. gentzenSequent NLP_Sequent Gamma C = natDed NLP_Sequent Gamma C``,
+    REPEAT STRIP_TAC
+ >> MP_TAC conditionOKNLP
+ >> REWRITE_TAC [gentzenEqNatDed]);
+
+(******************************************************************************)
+(*                                                                            *)
+(*                    Module: Arrow and Natural Deduction                     *)
+(*                                                                            *)
+(******************************************************************************)
+
+val natDedToArrow = store_thm (
+   "natDedToArrow",
+  ``!E X Gamma A. gentzenToArrowExt E X ==>
+                  natDed E Gamma A ==> arrow X (deltaTranslation Gamma) A``,
+    REPEAT STRIP_TAC
+ >> MATCH_MP_TAC gentzenToArrow
+ >> Q.EXISTS_TAC `E`
+ >> CONJ_TAC
+ >- ASM_REWRITE_TAC []
+ >> MATCH_MP_TAC natDedToGentzen
+ >> ASM_REWRITE_TAC []);
+
+val natDedToArrow_E = store_thm (
+   "natDedToArrow_E",
+  ``!E Gamma A. natDed E Gamma A ==> arrow (ToArrowExt E) (deltaTranslation Gamma) A``,
+    REPEAT GEN_TAC
+ >> MP_TAC (Q.SPEC `E` gentzenToArrowExt_thm)
+ >> REWRITE_TAC [natDedToArrow]);
+
+val arrowToNatDed = store_thm (
+   "arrowToNatDed",
+  ``!E X A B. condCutExt E /\ arrowToGentzenExt X E /\ arrow X A B
+	  ==> natDed E (OneForm A) B``,
+    REPEAT STRIP_TAC
+ >> irule gentzenToNatDed
+ >- ASM_REWRITE_TAC []
+ >> irule arrowToGentzen
+ >> Q.EXISTS_TAC `X`
+ >> ASM_REWRITE_TAC []);
+
+(******************************************************************************)
+(*                                                                            *)
+(*                          Grammar support in HOL                            *)
+(*                                                                            *)
+(******************************************************************************)
+
+fun enable_grammar () = let
+in
+    add_rule { term_name = "arrow", fixity = Infix (NONASSOC, 450),
+	pp_elements = [ HardSpace 0, TOK ":-", BreakSpace(1,0), TM, BreakSpace(1,0), TOK "-->",
+			BreakSpace(1,0) ],
+	paren_style = OnlyIfNecessary,
+	block_style = (AroundEachPhrase, (PP.CONSISTENT, 0)) };
+
+    add_rule { term_name = "natDed", fixity = Infix (NONASSOC, 450),
+	pp_elements = [ HardSpace 0, TOK ":-", BreakSpace(1,0), TM, BreakSpace(1,0), TOK "|-n",
+			BreakSpace(1,0) ],
+	paren_style = OnlyIfNecessary,
+	block_style = (AroundEachPhrase, (PP.CONSISTENT, 0)) };
+
+    add_rule { term_name = "gentzenSequent", fixity = Infix (NONASSOC, 450),
+	pp_elements = [ HardSpace 0, TOK ":-", BreakSpace(1,0), TM, BreakSpace(1,0), TOK "|-g",
+			BreakSpace(1,0) ],
+	paren_style = OnlyIfNecessary,
+	block_style = (AroundEachPhrase, (PP.CONSISTENT, 0)) }
+end;
+
+(* val _ = enable_grammar (); *)
 
 val _ = export_theory ();
+val _ = DB.html_theory "Lambek";
 
-(* last updated: January 18, 2017 *)
+(* last updated: April 10, 2017 *)
